Latest types for AWS KMS

src/AWS-KMS/Model/ComAmazonawsKmsTypes.dfy
@@ -13,11 +13,13 @@ include "../../StandardLibrary/StandardLibrary.dfy"
 	| RSAES_OAEP_SHA_1
 	| RSAES_OAEP_SHA_256
  type AliasList = seq<AliasListEntry>
- datatype AliasListEntry = AliasListEntry ( nameonly AliasName: Option<AliasNameType> ,
+ datatype AliasListEntry = | AliasListEntry (
+ nameonly AliasName: Option<AliasNameType> ,
  nameonly AliasArn: Option<ArnType> ,
  nameonly TargetKeyId: Option<KeyIdType> ,
  nameonly CreationDate: Option<string> ,
- nameonly LastUpdatedDate: Option<string> )
+ nameonly LastUpdatedDate: Option<string>
+ )
  type AliasNameType = x: string | IsValid_AliasNameType(x) witness *
  predicate method IsValid_AliasNameType(x: string) {
  ( 1 <= |x| <= 256 )
@@ -28,8 +30,12 @@ include "../../StandardLibrary/StandardLibrary.dfy"
 }
  type AWSAccountIdType = string
  type BooleanType = bool
- datatype CancelKeyDeletionRequest = CancelKeyDeletionRequest ( nameonly KeyId: KeyIdType )
- datatype CancelKeyDeletionResponse = CancelKeyDeletionResponse ( nameonly KeyId: Option<KeyIdType> )
+ datatype CancelKeyDeletionRequest = | CancelKeyDeletionRequest (
+ nameonly KeyId: KeyIdType
+ )
+ datatype CancelKeyDeletionResponse = | CancelKeyDeletionResponse (
+ nameonly KeyId: Option<KeyIdType>
+ )
  type CiphertextType = x: seq<uint8> | IsValid_CiphertextType(x) witness *
  predicate method IsValid_CiphertextType(x: seq<uint8>) {
  ( 1 <= |x| <= 6144 )
@@ -38,8 +44,12 @@ include "../../StandardLibrary/StandardLibrary.dfy"
  predicate method IsValid_CloudHsmClusterIdType(x: string) {
  ( 19 <= |x| <= 24 )
 }
- datatype ConnectCustomKeyStoreRequest = ConnectCustomKeyStoreRequest ( nameonly CustomKeyStoreId: CustomKeyStoreIdType )
- datatype ConnectCustomKeyStoreResponse = ConnectCustomKeyStoreResponse (  )
+ datatype ConnectCustomKeyStoreRequest = | ConnectCustomKeyStoreRequest (
+ nameonly CustomKeyStoreId: CustomKeyStoreIdType
+ )
+ datatype ConnectCustomKeyStoreResponse = | ConnectCustomKeyStoreResponse (
+ 
+ )
  datatype ConnectionErrorCodeType =
 	| INVALID_CREDENTIALS
 	| CLUSTER_NOT_FOUND
@@ -56,23 +66,34 @@ include "../../StandardLibrary/StandardLibrary.dfy"
 	| FAILED
 	| DISCONNECTED
 	| DISCONNECTING
- datatype CreateAliasRequest = CreateAliasRequest ( nameonly AliasName: AliasNameType ,
- nameonly TargetKeyId: KeyIdType )
- datatype CreateCustomKeyStoreRequest = CreateCustomKeyStoreRequest ( nameonly CustomKeyStoreName: CustomKeyStoreNameType ,
+ datatype CreateAliasRequest = | CreateAliasRequest (
+ nameonly AliasName: AliasNameType ,
+ nameonly TargetKeyId: KeyIdType
+ )
+ datatype CreateCustomKeyStoreRequest = | CreateCustomKeyStoreRequest (
+ nameonly CustomKeyStoreName: CustomKeyStoreNameType ,
  nameonly CloudHsmClusterId: CloudHsmClusterIdType ,
  nameonly TrustAnchorCertificate: TrustAnchorCertificateType ,
- nameonly KeyStorePassword: KeyStorePasswordType )
- datatype CreateCustomKeyStoreResponse = CreateCustomKeyStoreResponse ( nameonly CustomKeyStoreId: Option<CustomKeyStoreIdType> )
- datatype CreateGrantRequest = CreateGrantRequest ( nameonly KeyId: KeyIdType ,
+ nameonly KeyStorePassword: KeyStorePasswordType
+ )
+ datatype CreateCustomKeyStoreResponse = | CreateCustomKeyStoreResponse (
+ nameonly CustomKeyStoreId: Option<CustomKeyStoreIdType>
+ )
+ datatype CreateGrantRequest = | CreateGrantRequest (
+ nameonly KeyId: KeyIdType ,
  nameonly GranteePrincipal: PrincipalIdType ,
  nameonly RetiringPrincipal: Option<PrincipalIdType> ,
  nameonly Operations: GrantOperationList ,
  nameonly Constraints: Option<GrantConstraints> ,
  nameonly GrantTokens: Option<GrantTokenList> ,
- nameonly Name: Option<GrantNameType> )
- datatype CreateGrantResponse = CreateGrantResponse ( nameonly GrantToken: Option<GrantTokenType> ,
- nameonly GrantId: Option<GrantIdType> )
- datatype CreateKeyRequest = CreateKeyRequest ( nameonly Policy: Option<PolicyType> ,
+ nameonly Name: Option<GrantNameType>
+ )
+ datatype CreateGrantResponse = | CreateGrantResponse (
+ nameonly GrantToken: Option<GrantTokenType> ,
+ nameonly GrantId: Option<GrantIdType>
+ )
+ datatype CreateKeyRequest = | CreateKeyRequest (
+ nameonly Policy: Option<PolicyType> ,
  nameonly Description: Option<DescriptionType> ,
  nameonly KeyUsage: Option<KeyUsageType> ,
  nameonly CustomerMasterKeySpec: Option<CustomerMasterKeySpec> ,
@@ -81,8 +102,11 @@ include "../../StandardLibrary/StandardLibrary.dfy"
  nameonly CustomKeyStoreId: Option<CustomKeyStoreIdType> ,
  nameonly BypassPolicyLockoutSafetyCheck: Option<BooleanType> ,
  nameonly Tags: Option<TagList> ,
- nameonly MultiRegion: Option<NullableBooleanType> )
- datatype CreateKeyResponse = CreateKeyResponse ( nameonly KeyMetadata: Option<KeyMetadata> )
+ nameonly MultiRegion: Option<NullableBooleanType>
+ )
+ datatype CreateKeyResponse = | CreateKeyResponse (
+ nameonly KeyMetadata: Option<KeyMetadata>
+ )
  datatype CustomerMasterKeySpec =
 	| RSA_2048
 	| RSA_3072
@@ -101,13 +125,15 @@ include "../../StandardLibrary/StandardLibrary.dfy"
  ( 1 <= |x| <= 256 )
 }
  type CustomKeyStoresList = seq<CustomKeyStoresListEntry>
- datatype CustomKeyStoresListEntry = CustomKeyStoresListEntry ( nameonly CustomKeyStoreId: Option<CustomKeyStoreIdType> ,
+ datatype CustomKeyStoresListEntry = | CustomKeyStoresListEntry (
+ nameonly CustomKeyStoreId: Option<CustomKeyStoreIdType> ,
  nameonly CustomKeyStoreName: Option<CustomKeyStoreNameType> ,
  nameonly CloudHsmClusterId: Option<CloudHsmClusterIdType> ,
  nameonly TrustAnchorCertificate: Option<TrustAnchorCertificateType> ,
  nameonly ConnectionState: Option<ConnectionStateType> ,
  nameonly ConnectionErrorCode: Option<ConnectionErrorCodeType> ,
- nameonly CreationDate: Option<string> )
+ nameonly CreationDate: Option<string>
+ )
  datatype DataKeyPairSpec =
 	| RSA_2048
 	| RSA_3072
@@ -119,38 +145,70 @@ include "../../StandardLibrary/StandardLibrary.dfy"
  datatype DataKeySpec =
 	| AES_256
 	| AES_128
- datatype DecryptRequest = DecryptRequest ( nameonly CiphertextBlob: CiphertextType ,
+ datatype DecryptRequest = | DecryptRequest (
+ nameonly CiphertextBlob: CiphertextType ,
  nameonly EncryptionContext: Option<EncryptionContextType> ,
  nameonly GrantTokens: Option<GrantTokenList> ,
  nameonly KeyId: Option<KeyIdType> ,
- nameonly EncryptionAlgorithm: Option<EncryptionAlgorithmSpec> )
- datatype DecryptResponse = DecryptResponse ( nameonly KeyId: Option<KeyIdType> ,
+ nameonly EncryptionAlgorithm: Option<EncryptionAlgorithmSpec>
+ )
+ datatype DecryptResponse = | DecryptResponse (
+ nameonly KeyId: Option<KeyIdType> ,
  nameonly Plaintext: Option<PlaintextType> ,
- nameonly EncryptionAlgorithm: Option<EncryptionAlgorithmSpec> )
- datatype DeleteAliasRequest = DeleteAliasRequest ( nameonly AliasName: AliasNameType )
- datatype DeleteCustomKeyStoreRequest = DeleteCustomKeyStoreRequest ( nameonly CustomKeyStoreId: CustomKeyStoreIdType )
- datatype DeleteCustomKeyStoreResponse = DeleteCustomKeyStoreResponse (  )
- datatype DeleteImportedKeyMaterialRequest = DeleteImportedKeyMaterialRequest ( nameonly KeyId: KeyIdType )
- datatype DescribeCustomKeyStoresRequest = DescribeCustomKeyStoresRequest ( nameonly CustomKeyStoreId: Option<CustomKeyStoreIdType> ,
+ nameonly EncryptionAlgorithm: Option<EncryptionAlgorithmSpec>
+ )
+ datatype DeleteAliasRequest = | DeleteAliasRequest (
+ nameonly AliasName: AliasNameType
+ )
+ datatype DeleteCustomKeyStoreRequest = | DeleteCustomKeyStoreRequest (
+ nameonly CustomKeyStoreId: CustomKeyStoreIdType
+ )
+ datatype DeleteCustomKeyStoreResponse = | DeleteCustomKeyStoreResponse (
+ 
+ )
+ datatype DeleteImportedKeyMaterialRequest = | DeleteImportedKeyMaterialRequest (
+ nameonly KeyId: KeyIdType
+ )
+ datatype DescribeCustomKeyStoresRequest = | DescribeCustomKeyStoresRequest (
+ nameonly CustomKeyStoreId: Option<CustomKeyStoreIdType> ,
  nameonly CustomKeyStoreName: Option<CustomKeyStoreNameType> ,
  nameonly Limit: Option<LimitType> ,
- nameonly Marker: Option<MarkerType> )
- datatype DescribeCustomKeyStoresResponse = DescribeCustomKeyStoresResponse ( nameonly CustomKeyStores: Option<CustomKeyStoresList> ,
+ nameonly Marker: Option<MarkerType>
+ )
+ datatype DescribeCustomKeyStoresResponse = | DescribeCustomKeyStoresResponse (
+ nameonly CustomKeyStores: Option<CustomKeyStoresList> ,
  nameonly NextMarker: Option<MarkerType> ,
- nameonly Truncated: Option<BooleanType> )
- datatype DescribeKeyRequest = DescribeKeyRequest ( nameonly KeyId: KeyIdType ,
- nameonly GrantTokens: Option<GrantTokenList> )
- datatype DescribeKeyResponse = DescribeKeyResponse ( nameonly KeyMetadata: Option<KeyMetadata> )
+ nameonly Truncated: Option<BooleanType>
+ )
+ datatype DescribeKeyRequest = | DescribeKeyRequest (
+ nameonly KeyId: KeyIdType ,
+ nameonly GrantTokens: Option<GrantTokenList>
+ )
+ datatype DescribeKeyResponse = | DescribeKeyResponse (
+ nameonly KeyMetadata: Option<KeyMetadata>
+ )
  type DescriptionType = x: string | IsValid_DescriptionType(x) witness *
  predicate method IsValid_DescriptionType(x: string) {
  ( 0 <= |x| <= 8192 )
 }
- datatype DisableKeyRequest = DisableKeyRequest ( nameonly KeyId: KeyIdType )
- datatype DisableKeyRotationRequest = DisableKeyRotationRequest ( nameonly KeyId: KeyIdType )
- datatype DisconnectCustomKeyStoreRequest = DisconnectCustomKeyStoreRequest ( nameonly CustomKeyStoreId: CustomKeyStoreIdType )
- datatype DisconnectCustomKeyStoreResponse = DisconnectCustomKeyStoreResponse (  )
- datatype EnableKeyRequest = EnableKeyRequest ( nameonly KeyId: KeyIdType )
- datatype EnableKeyRotationRequest = EnableKeyRotationRequest ( nameonly KeyId: KeyIdType )
+ datatype DisableKeyRequest = | DisableKeyRequest (
+ nameonly KeyId: KeyIdType
+ )
+ datatype DisableKeyRotationRequest = | DisableKeyRotationRequest (
+ nameonly KeyId: KeyIdType
+ )
+ datatype DisconnectCustomKeyStoreRequest = | DisconnectCustomKeyStoreRequest (
+ nameonly CustomKeyStoreId: CustomKeyStoreIdType
+ )
+ datatype DisconnectCustomKeyStoreResponse = | DisconnectCustomKeyStoreResponse (
+ 
+ )
+ datatype EnableKeyRequest = | EnableKeyRequest (
+ nameonly KeyId: KeyIdType
+ )
+ datatype EnableKeyRotationRequest = | EnableKeyRotationRequest (
+ nameonly KeyId: KeyIdType
+ )
  datatype EncryptionAlgorithmSpec =
 	| SYMMETRIC_DEFAULT
 	| RSAES_OAEP_SHA_1
@@ -159,82 +217,125 @@ include "../../StandardLibrary/StandardLibrary.dfy"
  type EncryptionContextKey = string
  type EncryptionContextType = map<EncryptionContextKey, EncryptionContextValue>
  type EncryptionContextValue = string
- datatype EncryptRequest = EncryptRequest ( nameonly KeyId: KeyIdType ,
+ datatype EncryptRequest = | EncryptRequest (
+ nameonly KeyId: KeyIdType ,
  nameonly Plaintext: PlaintextType ,
  nameonly EncryptionContext: Option<EncryptionContextType> ,
  nameonly GrantTokens: Option<GrantTokenList> ,
- nameonly EncryptionAlgorithm: Option<EncryptionAlgorithmSpec> )
- datatype EncryptResponse = EncryptResponse ( nameonly CiphertextBlob: Option<CiphertextType> ,
+ nameonly EncryptionAlgorithm: Option<EncryptionAlgorithmSpec>
+ )
+ datatype EncryptResponse = | EncryptResponse (
+ nameonly CiphertextBlob: Option<CiphertextType> ,
  nameonly KeyId: Option<KeyIdType> ,
- nameonly EncryptionAlgorithm: Option<EncryptionAlgorithmSpec> )
+ nameonly EncryptionAlgorithm: Option<EncryptionAlgorithmSpec>
+ )
  type ErrorMessageType = string
  datatype ExpirationModelType =
 	| KEY_MATERIAL_EXPIRES
 	| KEY_MATERIAL_DOES_NOT_EXPIRE
- datatype GenerateDataKeyPairRequest = GenerateDataKeyPairRequest ( nameonly EncryptionContext: Option<EncryptionContextType> ,
+ datatype GenerateDataKeyPairRequest = | GenerateDataKeyPairRequest (
+ nameonly EncryptionContext: Option<EncryptionContextType> ,
  nameonly KeyId: KeyIdType ,
  nameonly KeyPairSpec: DataKeyPairSpec ,
- nameonly GrantTokens: Option<GrantTokenList> )
- datatype GenerateDataKeyPairResponse = GenerateDataKeyPairResponse ( nameonly PrivateKeyCiphertextBlob: Option<CiphertextType> ,
+ nameonly GrantTokens: Option<GrantTokenList>
+ )
+ datatype GenerateDataKeyPairResponse = | GenerateDataKeyPairResponse (
+ nameonly PrivateKeyCiphertextBlob: Option<CiphertextType> ,
  nameonly PrivateKeyPlaintext: Option<PlaintextType> ,
  nameonly PublicKey: Option<PublicKeyType> ,
  nameonly KeyId: Option<KeyIdType> ,
- nameonly KeyPairSpec: Option<DataKeyPairSpec> )
- datatype GenerateDataKeyPairWithoutPlaintextRequest = GenerateDataKeyPairWithoutPlaintextRequest ( nameonly EncryptionContext: Option<EncryptionContextType> ,
+ nameonly KeyPairSpec: Option<DataKeyPairSpec>
+ )
+ datatype GenerateDataKeyPairWithoutPlaintextRequest = | GenerateDataKeyPairWithoutPlaintextRequest (
+ nameonly EncryptionContext: Option<EncryptionContextType> ,
  nameonly KeyId: KeyIdType ,
  nameonly KeyPairSpec: DataKeyPairSpec ,
- nameonly GrantTokens: Option<GrantTokenList> )
- datatype GenerateDataKeyPairWithoutPlaintextResponse = GenerateDataKeyPairWithoutPlaintextResponse ( nameonly PrivateKeyCiphertextBlob: Option<CiphertextType> ,
+ nameonly GrantTokens: Option<GrantTokenList>
+ )
+ datatype GenerateDataKeyPairWithoutPlaintextResponse = | GenerateDataKeyPairWithoutPlaintextResponse (
+ nameonly PrivateKeyCiphertextBlob: Option<CiphertextType> ,
  nameonly PublicKey: Option<PublicKeyType> ,
  nameonly KeyId: Option<KeyIdType> ,
- nameonly KeyPairSpec: Option<DataKeyPairSpec> )
- datatype GenerateDataKeyRequest = GenerateDataKeyRequest ( nameonly KeyId: KeyIdType ,
+ nameonly KeyPairSpec: Option<DataKeyPairSpec>
+ )
+ datatype GenerateDataKeyRequest = | GenerateDataKeyRequest (
+ nameonly KeyId: KeyIdType ,
  nameonly EncryptionContext: Option<EncryptionContextType> ,
  nameonly NumberOfBytes: Option<NumberOfBytesType> ,
  nameonly KeySpec: Option<DataKeySpec> ,
- nameonly GrantTokens: Option<GrantTokenList> )
- datatype GenerateDataKeyResponse = GenerateDataKeyResponse ( nameonly CiphertextBlob: Option<CiphertextType> ,
+ nameonly GrantTokens: Option<GrantTokenList>
+ )
+ datatype GenerateDataKeyResponse = | GenerateDataKeyResponse (
+ nameonly CiphertextBlob: Option<CiphertextType> ,
  nameonly Plaintext: Option<PlaintextType> ,
- nameonly KeyId: Option<KeyIdType> )
- datatype GenerateDataKeyWithoutPlaintextRequest = GenerateDataKeyWithoutPlaintextRequest ( nameonly KeyId: KeyIdType ,
+ nameonly KeyId: Option<KeyIdType>
+ )
+ datatype GenerateDataKeyWithoutPlaintextRequest = | GenerateDataKeyWithoutPlaintextRequest (
+ nameonly KeyId: KeyIdType ,
  nameonly EncryptionContext: Option<EncryptionContextType> ,
  nameonly KeySpec: Option<DataKeySpec> ,
  nameonly NumberOfBytes: Option<NumberOfBytesType> ,
- nameonly GrantTokens: Option<GrantTokenList> )
- datatype GenerateDataKeyWithoutPlaintextResponse = GenerateDataKeyWithoutPlaintextResponse ( nameonly CiphertextBlob: Option<CiphertextType> ,
- nameonly KeyId: Option<KeyIdType> )
- datatype GenerateRandomRequest = GenerateRandomRequest ( nameonly NumberOfBytes: Option<NumberOfBytesType> ,
- nameonly CustomKeyStoreId: Option<CustomKeyStoreIdType> )
- datatype GenerateRandomResponse = GenerateRandomResponse ( nameonly Plaintext: Option<PlaintextType> )
- datatype GetKeyPolicyRequest = GetKeyPolicyRequest ( nameonly KeyId: KeyIdType ,
- nameonly PolicyName: PolicyNameType )
- datatype GetKeyPolicyResponse = GetKeyPolicyResponse ( nameonly Policy: Option<PolicyType> )
- datatype GetKeyRotationStatusRequest = GetKeyRotationStatusRequest ( nameonly KeyId: KeyIdType )
- datatype GetKeyRotationStatusResponse = GetKeyRotationStatusResponse ( nameonly KeyRotationEnabled: Option<BooleanType> )
- datatype GetParametersForImportRequest = GetParametersForImportRequest ( nameonly KeyId: KeyIdType ,
+ nameonly GrantTokens: Option<GrantTokenList>
+ )
+ datatype GenerateDataKeyWithoutPlaintextResponse = | GenerateDataKeyWithoutPlaintextResponse (
+ nameonly CiphertextBlob: Option<CiphertextType> ,
+ nameonly KeyId: Option<KeyIdType>
+ )
+ datatype GenerateRandomRequest = | GenerateRandomRequest (
+ nameonly NumberOfBytes: Option<NumberOfBytesType> ,
+ nameonly CustomKeyStoreId: Option<CustomKeyStoreIdType>
+ )
+ datatype GenerateRandomResponse = | GenerateRandomResponse (
+ nameonly Plaintext: Option<PlaintextType>
+ )
+ datatype GetKeyPolicyRequest = | GetKeyPolicyRequest (
+ nameonly KeyId: KeyIdType ,
+ nameonly PolicyName: PolicyNameType
+ )
+ datatype GetKeyPolicyResponse = | GetKeyPolicyResponse (
+ nameonly Policy: Option<PolicyType>
+ )
+ datatype GetKeyRotationStatusRequest = | GetKeyRotationStatusRequest (
+ nameonly KeyId: KeyIdType
+ )
+ datatype GetKeyRotationStatusResponse = | GetKeyRotationStatusResponse (
+ nameonly KeyRotationEnabled: Option<BooleanType>
+ )
+ datatype GetParametersForImportRequest = | GetParametersForImportRequest (
+ nameonly KeyId: KeyIdType ,
  nameonly WrappingAlgorithm: AlgorithmSpec ,
- nameonly WrappingKeySpec: WrappingKeySpec )
- datatype GetParametersForImportResponse = GetParametersForImportResponse ( nameonly KeyId: Option<KeyIdType> ,
+ nameonly WrappingKeySpec: WrappingKeySpec
+ )
+ datatype GetParametersForImportResponse = | GetParametersForImportResponse (
+ nameonly KeyId: Option<KeyIdType> ,
  nameonly ImportToken: Option<CiphertextType> ,
  nameonly PublicKey: Option<PlaintextType> ,
- nameonly ParametersValidTo: Option<string> )
- datatype GetPublicKeyRequest = GetPublicKeyRequest ( nameonly KeyId: KeyIdType ,
- nameonly GrantTokens: Option<GrantTokenList> )
- datatype GetPublicKeyResponse = GetPublicKeyResponse ( nameonly KeyId: Option<KeyIdType> ,
+ nameonly ParametersValidTo: Option<string>
+ )
+ datatype GetPublicKeyRequest = | GetPublicKeyRequest (
+ nameonly KeyId: KeyIdType ,
+ nameonly GrantTokens: Option<GrantTokenList>
+ )
+ datatype GetPublicKeyResponse = | GetPublicKeyResponse (
+ nameonly KeyId: Option<KeyIdType> ,
  nameonly PublicKey: Option<PublicKeyType> ,
  nameonly CustomerMasterKeySpec: Option<CustomerMasterKeySpec> ,
  nameonly KeySpec: Option<KeySpec> ,
  nameonly KeyUsage: Option<KeyUsageType> ,
  nameonly EncryptionAlgorithms: Option<EncryptionAlgorithmSpecList> ,
- nameonly SigningAlgorithms: Option<SigningAlgorithmSpecList> )
- datatype GrantConstraints = GrantConstraints ( nameonly EncryptionContextSubset: Option<EncryptionContextType> ,
- nameonly EncryptionContextEquals: Option<EncryptionContextType> )
+ nameonly SigningAlgorithms: Option<SigningAlgorithmSpecList>
+ )
+ datatype GrantConstraints = | GrantConstraints (
+ nameonly EncryptionContextSubset: Option<EncryptionContextType> ,
+ nameonly EncryptionContextEquals: Option<EncryptionContextType>
+ )
  type GrantIdType = x: string | IsValid_GrantIdType(x) witness *
  predicate method IsValid_GrantIdType(x: string) {
  ( 1 <= |x| <= 128 )
 }
  type GrantList = seq<GrantListEntry>
- datatype GrantListEntry = GrantListEntry ( nameonly KeyId: Option<KeyIdType> ,
+ datatype GrantListEntry = | GrantListEntry (
+ nameonly KeyId: Option<KeyIdType> ,
  nameonly GrantId: Option<GrantIdType> ,
  nameonly Name: Option<GrantNameType> ,
  nameonly CreationDate: Option<string> ,
@@ -242,7 +343,8 @@ include "../../StandardLibrary/StandardLibrary.dfy"
  nameonly RetiringPrincipal: Option<PrincipalIdType> ,
  nameonly IssuingAccount: Option<PrincipalIdType> ,
  nameonly Operations: Option<GrantOperationList> ,
- nameonly Constraints: Option<GrantConstraints> )
+ nameonly Constraints: Option<GrantConstraints>
+ )
  type GrantNameType = x: string | IsValid_GrantNameType(x) witness *
  predicate method IsValid_GrantNameType(x: string) {
  ( 1 <= |x| <= 256 )
@@ -271,293 +373,299 @@ include "../../StandardLibrary/StandardLibrary.dfy"
  predicate method IsValid_GrantTokenType(x: string) {
  ( 1 <= |x| <= 8192 )
 }
- datatype ImportKeyMaterialRequest = ImportKeyMaterialRequest ( nameonly KeyId: KeyIdType ,
+ datatype ImportKeyMaterialRequest = | ImportKeyMaterialRequest (
+ nameonly KeyId: KeyIdType ,
  nameonly ImportToken: CiphertextType ,
  nameonly EncryptedKeyMaterial: CiphertextType ,
  nameonly ValidTo: Option<string> ,
- nameonly ExpirationModel: Option<ExpirationModelType> )
- datatype ImportKeyMaterialResponse = ImportKeyMaterialResponse (  )
+ nameonly ExpirationModel: Option<ExpirationModelType>
+ )
+ datatype ImportKeyMaterialResponse = | ImportKeyMaterialResponse (
+ 
+ )
  type KeyIdType = x: string | IsValid_KeyIdType(x) witness *
  predicate method IsValid_KeyIdType(x: string) {
  ( 1 <= |x| <= 2048 )
 }
  type KeyList = seq<KeyListEntry>
- datatype KeyListEntry = KeyListEntry ( nameonly KeyId: Option<KeyIdType> ,
- nameonly KeyArn: Option<ArnType> )
+ datatype KeyListEntry = | KeyListEntry (
+ nameonly KeyId: Option<KeyIdType> ,
+ nameonly KeyArn: Option<ArnType>
+ )
  trait {:termination false} IKeyManagementServiceClient {
- predicate CancelKeyDeletionCalledWith ( input: CancelKeyDeletionRequest ) {true}
- predicate CancelKeyDeletionSucceededWith (  input: CancelKeyDeletionRequest , output: CancelKeyDeletionResponse ) {true}
- method CancelKeyDeletion ( input: CancelKeyDeletionRequest ) returns  ( output: Result<CancelKeyDeletionResponse, Error> )
+ predicate {:opaque} CancelKeyDeletionCalledWith ( input: CancelKeyDeletionRequest ) {true}
+ predicate {:opaque} CancelKeyDeletionSucceededWith (  input: CancelKeyDeletionRequest , output: CancelKeyDeletionResponse ) {true}
+ method CancelKeyDeletion ( input: CancelKeyDeletionRequest ) returns (output: Result<CancelKeyDeletionResponse, Error>)
 	ensures CancelKeyDeletionCalledWith (  input )
 	ensures output.Success? ==> CancelKeyDeletionSucceededWith (  input , output.value )
 
- predicate ConnectCustomKeyStoreCalledWith ( input: ConnectCustomKeyStoreRequest ) {true}
- predicate ConnectCustomKeyStoreSucceededWith (  input: ConnectCustomKeyStoreRequest , output: ConnectCustomKeyStoreResponse ) {true}
- method ConnectCustomKeyStore ( input: ConnectCustomKeyStoreRequest ) returns  ( output: Result<ConnectCustomKeyStoreResponse, Error> )
+ predicate {:opaque} ConnectCustomKeyStoreCalledWith ( input: ConnectCustomKeyStoreRequest ) {true}
+ predicate {:opaque} ConnectCustomKeyStoreSucceededWith (  input: ConnectCustomKeyStoreRequest , output: ConnectCustomKeyStoreResponse ) {true}
+ method ConnectCustomKeyStore ( input: ConnectCustomKeyStoreRequest ) returns (output: Result<ConnectCustomKeyStoreResponse, Error>)
 	ensures ConnectCustomKeyStoreCalledWith (  input )
 	ensures output.Success? ==> ConnectCustomKeyStoreSucceededWith (  input , output.value )
 
- predicate CreateAliasCalledWith ( input: CreateAliasRequest ) {true}
- predicate CreateAliasSucceededWith (  input: CreateAliasRequest ) {true}
- method CreateAlias ( input: CreateAliasRequest ) returns  ( output: Result<(), Error> )
+ predicate {:opaque} CreateAliasCalledWith ( input: CreateAliasRequest ) {true}
+ predicate {:opaque} CreateAliasSucceededWith (  input: CreateAliasRequest ) {true}
+ method CreateAlias ( input: CreateAliasRequest ) returns (output: Result<(), Error>)
 	ensures CreateAliasCalledWith (  input )
 	ensures output.Success? ==> CreateAliasSucceededWith (  input )
 
- predicate CreateCustomKeyStoreCalledWith ( input: CreateCustomKeyStoreRequest ) {true}
- predicate CreateCustomKeyStoreSucceededWith (  input: CreateCustomKeyStoreRequest , output: CreateCustomKeyStoreResponse ) {true}
- method CreateCustomKeyStore ( input: CreateCustomKeyStoreRequest ) returns  ( output: Result<CreateCustomKeyStoreResponse, Error> )
+ predicate {:opaque} CreateCustomKeyStoreCalledWith ( input: CreateCustomKeyStoreRequest ) {true}
+ predicate {:opaque} CreateCustomKeyStoreSucceededWith (  input: CreateCustomKeyStoreRequest , output: CreateCustomKeyStoreResponse ) {true}
+ method CreateCustomKeyStore ( input: CreateCustomKeyStoreRequest ) returns (output: Result<CreateCustomKeyStoreResponse, Error>)
 	ensures CreateCustomKeyStoreCalledWith (  input )
 	ensures output.Success? ==> CreateCustomKeyStoreSucceededWith (  input , output.value )
 
- predicate CreateGrantCalledWith ( input: CreateGrantRequest ) {true}
- predicate CreateGrantSucceededWith (  input: CreateGrantRequest , output: CreateGrantResponse ) {true}
- method CreateGrant ( input: CreateGrantRequest ) returns  ( output: Result<CreateGrantResponse, Error> )
+ predicate {:opaque} CreateGrantCalledWith ( input: CreateGrantRequest ) {true}
+ predicate {:opaque} CreateGrantSucceededWith (  input: CreateGrantRequest , output: CreateGrantResponse ) {true}
+ method CreateGrant ( input: CreateGrantRequest ) returns (output: Result<CreateGrantResponse, Error>)
 	ensures CreateGrantCalledWith (  input )
 	ensures output.Success? ==> CreateGrantSucceededWith (  input , output.value )
 
- predicate CreateKeyCalledWith ( input: CreateKeyRequest ) {true}
- predicate CreateKeySucceededWith (  input: CreateKeyRequest , output: CreateKeyResponse ) {true}
- method CreateKey ( input: CreateKeyRequest ) returns  ( output: Result<CreateKeyResponse, Error> )
+ predicate {:opaque} CreateKeyCalledWith ( input: CreateKeyRequest ) {true}
+ predicate {:opaque} CreateKeySucceededWith (  input: CreateKeyRequest , output: CreateKeyResponse ) {true}
+ method CreateKey ( input: CreateKeyRequest ) returns (output: Result<CreateKeyResponse, Error>)
 	ensures CreateKeyCalledWith (  input )
 	ensures output.Success? ==> CreateKeySucceededWith (  input , output.value )
 
- predicate DecryptCalledWith ( input: DecryptRequest ) {true}
- predicate DecryptSucceededWith (  input: DecryptRequest , output: DecryptResponse ) {true}
- method Decrypt ( input: DecryptRequest ) returns  ( output: Result<DecryptResponse, Error> )
+ predicate {:opaque} DecryptCalledWith ( input: DecryptRequest ) {true}
+ predicate {:opaque} DecryptSucceededWith (  input: DecryptRequest , output: DecryptResponse ) {true}
+ method Decrypt ( input: DecryptRequest ) returns (output: Result<DecryptResponse, Error>)
 	ensures DecryptCalledWith (  input )
 	ensures output.Success? ==> DecryptSucceededWith (  input , output.value )
 
- predicate DeleteAliasCalledWith ( input: DeleteAliasRequest ) {true}
- predicate DeleteAliasSucceededWith (  input: DeleteAliasRequest ) {true}
- method DeleteAlias ( input: DeleteAliasRequest ) returns  ( output: Result<(), Error> )
+ predicate {:opaque} DeleteAliasCalledWith ( input: DeleteAliasRequest ) {true}
+ predicate {:opaque} DeleteAliasSucceededWith (  input: DeleteAliasRequest ) {true}
+ method DeleteAlias ( input: DeleteAliasRequest ) returns (output: Result<(), Error>)
 	ensures DeleteAliasCalledWith (  input )
 	ensures output.Success? ==> DeleteAliasSucceededWith (  input )
 
- predicate DeleteCustomKeyStoreCalledWith ( input: DeleteCustomKeyStoreRequest ) {true}
- predicate DeleteCustomKeyStoreSucceededWith (  input: DeleteCustomKeyStoreRequest , output: DeleteCustomKeyStoreResponse ) {true}
- method DeleteCustomKeyStore ( input: DeleteCustomKeyStoreRequest ) returns  ( output: Result<DeleteCustomKeyStoreResponse, Error> )
+ predicate {:opaque} DeleteCustomKeyStoreCalledWith ( input: DeleteCustomKeyStoreRequest ) {true}
+ predicate {:opaque} DeleteCustomKeyStoreSucceededWith (  input: DeleteCustomKeyStoreRequest , output: DeleteCustomKeyStoreResponse ) {true}
+ method DeleteCustomKeyStore ( input: DeleteCustomKeyStoreRequest ) returns (output: Result<DeleteCustomKeyStoreResponse, Error>)
 	ensures DeleteCustomKeyStoreCalledWith (  input )
 	ensures output.Success? ==> DeleteCustomKeyStoreSucceededWith (  input , output.value )
 
- predicate DeleteImportedKeyMaterialCalledWith ( input: DeleteImportedKeyMaterialRequest ) {true}
- predicate DeleteImportedKeyMaterialSucceededWith (  input: DeleteImportedKeyMaterialRequest ) {true}
- method DeleteImportedKeyMaterial ( input: DeleteImportedKeyMaterialRequest ) returns  ( output: Result<(), Error> )
+ predicate {:opaque} DeleteImportedKeyMaterialCalledWith ( input: DeleteImportedKeyMaterialRequest ) {true}
+ predicate {:opaque} DeleteImportedKeyMaterialSucceededWith (  input: DeleteImportedKeyMaterialRequest ) {true}
+ method DeleteImportedKeyMaterial ( input: DeleteImportedKeyMaterialRequest ) returns (output: Result<(), Error>)
 	ensures DeleteImportedKeyMaterialCalledWith (  input )
 	ensures output.Success? ==> DeleteImportedKeyMaterialSucceededWith (  input )
 
- predicate DescribeCustomKeyStoresCalledWith ( input: DescribeCustomKeyStoresRequest ) {true}
- predicate DescribeCustomKeyStoresSucceededWith (  input: DescribeCustomKeyStoresRequest , output: DescribeCustomKeyStoresResponse ) {true}
- method DescribeCustomKeyStores ( input: DescribeCustomKeyStoresRequest ) returns  ( output: Result<DescribeCustomKeyStoresResponse, Error> )
+ predicate {:opaque} DescribeCustomKeyStoresCalledWith ( input: DescribeCustomKeyStoresRequest ) {true}
+ predicate {:opaque} DescribeCustomKeyStoresSucceededWith (  input: DescribeCustomKeyStoresRequest , output: DescribeCustomKeyStoresResponse ) {true}
+ method DescribeCustomKeyStores ( input: DescribeCustomKeyStoresRequest ) returns (output: Result<DescribeCustomKeyStoresResponse, Error>)
 	ensures DescribeCustomKeyStoresCalledWith (  input )
 	ensures output.Success? ==> DescribeCustomKeyStoresSucceededWith (  input , output.value )
 
- predicate DescribeKeyCalledWith ( input: DescribeKeyRequest ) {true}
- predicate DescribeKeySucceededWith (  input: DescribeKeyRequest , output: DescribeKeyResponse ) {true}
- method DescribeKey ( input: DescribeKeyRequest ) returns  ( output: Result<DescribeKeyResponse, Error> )
+ predicate {:opaque} DescribeKeyCalledWith ( input: DescribeKeyRequest ) {true}
+ predicate {:opaque} DescribeKeySucceededWith (  input: DescribeKeyRequest , output: DescribeKeyResponse ) {true}
+ method DescribeKey ( input: DescribeKeyRequest ) returns (output: Result<DescribeKeyResponse, Error>)
 	ensures DescribeKeyCalledWith (  input )
 	ensures output.Success? ==> DescribeKeySucceededWith (  input , output.value )
 
- predicate DisableKeyCalledWith ( input: DisableKeyRequest ) {true}
- predicate DisableKeySucceededWith (  input: DisableKeyRequest ) {true}
- method DisableKey ( input: DisableKeyRequest ) returns  ( output: Result<(), Error> )
+ predicate {:opaque} DisableKeyCalledWith ( input: DisableKeyRequest ) {true}
+ predicate {:opaque} DisableKeySucceededWith (  input: DisableKeyRequest ) {true}
+ method DisableKey ( input: DisableKeyRequest ) returns (output: Result<(), Error>)
 	ensures DisableKeyCalledWith (  input )
 	ensures output.Success? ==> DisableKeySucceededWith (  input )
 
- predicate DisableKeyRotationCalledWith ( input: DisableKeyRotationRequest ) {true}
- predicate DisableKeyRotationSucceededWith (  input: DisableKeyRotationRequest ) {true}
- method DisableKeyRotation ( input: DisableKeyRotationRequest ) returns  ( output: Result<(), Error> )
+ predicate {:opaque} DisableKeyRotationCalledWith ( input: DisableKeyRotationRequest ) {true}
+ predicate {:opaque} DisableKeyRotationSucceededWith (  input: DisableKeyRotationRequest ) {true}
+ method DisableKeyRotation ( input: DisableKeyRotationRequest ) returns (output: Result<(), Error>)
 	ensures DisableKeyRotationCalledWith (  input )
 	ensures output.Success? ==> DisableKeyRotationSucceededWith (  input )
 
- predicate DisconnectCustomKeyStoreCalledWith ( input: DisconnectCustomKeyStoreRequest ) {true}
- predicate DisconnectCustomKeyStoreSucceededWith (  input: DisconnectCustomKeyStoreRequest , output: DisconnectCustomKeyStoreResponse ) {true}
- method DisconnectCustomKeyStore ( input: DisconnectCustomKeyStoreRequest ) returns  ( output: Result<DisconnectCustomKeyStoreResponse, Error> )
+ predicate {:opaque} DisconnectCustomKeyStoreCalledWith ( input: DisconnectCustomKeyStoreRequest ) {true}
+ predicate {:opaque} DisconnectCustomKeyStoreSucceededWith (  input: DisconnectCustomKeyStoreRequest , output: DisconnectCustomKeyStoreResponse ) {true}
+ method DisconnectCustomKeyStore ( input: DisconnectCustomKeyStoreRequest ) returns (output: Result<DisconnectCustomKeyStoreResponse, Error>)
 	ensures DisconnectCustomKeyStoreCalledWith (  input )
 	ensures output.Success? ==> DisconnectCustomKeyStoreSucceededWith (  input , output.value )
 
- predicate EnableKeyCalledWith ( input: EnableKeyRequest ) {true}
- predicate EnableKeySucceededWith (  input: EnableKeyRequest ) {true}
- method EnableKey ( input: EnableKeyRequest ) returns  ( output: Result<(), Error> )
+ predicate {:opaque} EnableKeyCalledWith ( input: EnableKeyRequest ) {true}
+ predicate {:opaque} EnableKeySucceededWith (  input: EnableKeyRequest ) {true}
+ method EnableKey ( input: EnableKeyRequest ) returns (output: Result<(), Error>)
 	ensures EnableKeyCalledWith (  input )
 	ensures output.Success? ==> EnableKeySucceededWith (  input )
 
- predicate EnableKeyRotationCalledWith ( input: EnableKeyRotationRequest ) {true}
- predicate EnableKeyRotationSucceededWith (  input: EnableKeyRotationRequest ) {true}
- method EnableKeyRotation ( input: EnableKeyRotationRequest ) returns  ( output: Result<(), Error> )
+ predicate {:opaque} EnableKeyRotationCalledWith ( input: EnableKeyRotationRequest ) {true}
+ predicate {:opaque} EnableKeyRotationSucceededWith (  input: EnableKeyRotationRequest ) {true}
+ method EnableKeyRotation ( input: EnableKeyRotationRequest ) returns (output: Result<(), Error>)
 	ensures EnableKeyRotationCalledWith (  input )
 	ensures output.Success? ==> EnableKeyRotationSucceededWith (  input )
 
- predicate EncryptCalledWith ( input: EncryptRequest ) {true}
- predicate EncryptSucceededWith (  input: EncryptRequest , output: EncryptResponse ) {true}
- method Encrypt ( input: EncryptRequest ) returns  ( output: Result<EncryptResponse, Error> )
+ predicate {:opaque} EncryptCalledWith ( input: EncryptRequest ) {true}
+ predicate {:opaque} EncryptSucceededWith (  input: EncryptRequest , output: EncryptResponse ) {true}
+ method Encrypt ( input: EncryptRequest ) returns (output: Result<EncryptResponse, Error>)
 	ensures EncryptCalledWith (  input )
 	ensures output.Success? ==> EncryptSucceededWith (  input , output.value )
 
- predicate GenerateDataKeyCalledWith ( input: GenerateDataKeyRequest ) {true}
- predicate GenerateDataKeySucceededWith (  input: GenerateDataKeyRequest , output: GenerateDataKeyResponse ) {true}
- method GenerateDataKey ( input: GenerateDataKeyRequest ) returns  ( output: Result<GenerateDataKeyResponse, Error> )
+ predicate {:opaque} GenerateDataKeyCalledWith ( input: GenerateDataKeyRequest ) {true}
+ predicate {:opaque} GenerateDataKeySucceededWith (  input: GenerateDataKeyRequest , output: GenerateDataKeyResponse ) {true}
+ method GenerateDataKey ( input: GenerateDataKeyRequest ) returns (output: Result<GenerateDataKeyResponse, Error>)
 	ensures GenerateDataKeyCalledWith (  input )
 	ensures output.Success? ==> GenerateDataKeySucceededWith (  input , output.value )
 
- predicate GenerateDataKeyPairCalledWith ( input: GenerateDataKeyPairRequest ) {true}
- predicate GenerateDataKeyPairSucceededWith (  input: GenerateDataKeyPairRequest , output: GenerateDataKeyPairResponse ) {true}
- method GenerateDataKeyPair ( input: GenerateDataKeyPairRequest ) returns  ( output: Result<GenerateDataKeyPairResponse, Error> )
+ predicate {:opaque} GenerateDataKeyPairCalledWith ( input: GenerateDataKeyPairRequest ) {true}
+ predicate {:opaque} GenerateDataKeyPairSucceededWith (  input: GenerateDataKeyPairRequest , output: GenerateDataKeyPairResponse ) {true}
+ method GenerateDataKeyPair ( input: GenerateDataKeyPairRequest ) returns (output: Result<GenerateDataKeyPairResponse, Error>)
 	ensures GenerateDataKeyPairCalledWith (  input )
 	ensures output.Success? ==> GenerateDataKeyPairSucceededWith (  input , output.value )
 
- predicate GenerateDataKeyPairWithoutPlaintextCalledWith ( input: GenerateDataKeyPairWithoutPlaintextRequest ) {true}
- predicate GenerateDataKeyPairWithoutPlaintextSucceededWith (  input: GenerateDataKeyPairWithoutPlaintextRequest , output: GenerateDataKeyPairWithoutPlaintextResponse ) {true}
- method GenerateDataKeyPairWithoutPlaintext ( input: GenerateDataKeyPairWithoutPlaintextRequest ) returns  ( output: Result<GenerateDataKeyPairWithoutPlaintextResponse, Error> )
+ predicate {:opaque} GenerateDataKeyPairWithoutPlaintextCalledWith ( input: GenerateDataKeyPairWithoutPlaintextRequest ) {true}
+ predicate {:opaque} GenerateDataKeyPairWithoutPlaintextSucceededWith (  input: GenerateDataKeyPairWithoutPlaintextRequest , output: GenerateDataKeyPairWithoutPlaintextResponse ) {true}
+ method GenerateDataKeyPairWithoutPlaintext ( input: GenerateDataKeyPairWithoutPlaintextRequest ) returns (output: Result<GenerateDataKeyPairWithoutPlaintextResponse, Error>)
 	ensures GenerateDataKeyPairWithoutPlaintextCalledWith (  input )
 	ensures output.Success? ==> GenerateDataKeyPairWithoutPlaintextSucceededWith (  input , output.value )
 
- predicate GenerateDataKeyWithoutPlaintextCalledWith ( input: GenerateDataKeyWithoutPlaintextRequest ) {true}
- predicate GenerateDataKeyWithoutPlaintextSucceededWith (  input: GenerateDataKeyWithoutPlaintextRequest , output: GenerateDataKeyWithoutPlaintextResponse ) {true}
- method GenerateDataKeyWithoutPlaintext ( input: GenerateDataKeyWithoutPlaintextRequest ) returns  ( output: Result<GenerateDataKeyWithoutPlaintextResponse, Error> )
+ predicate {:opaque} GenerateDataKeyWithoutPlaintextCalledWith ( input: GenerateDataKeyWithoutPlaintextRequest ) {true}
+ predicate {:opaque} GenerateDataKeyWithoutPlaintextSucceededWith (  input: GenerateDataKeyWithoutPlaintextRequest , output: GenerateDataKeyWithoutPlaintextResponse ) {true}
+ method GenerateDataKeyWithoutPlaintext ( input: GenerateDataKeyWithoutPlaintextRequest ) returns (output: Result<GenerateDataKeyWithoutPlaintextResponse, Error>)
 	ensures GenerateDataKeyWithoutPlaintextCalledWith (  input )
 	ensures output.Success? ==> GenerateDataKeyWithoutPlaintextSucceededWith (  input , output.value )
 
- predicate GenerateRandomCalledWith ( input: GenerateRandomRequest ) {true}
- predicate GenerateRandomSucceededWith (  input: GenerateRandomRequest , output: GenerateRandomResponse ) {true}
- method GenerateRandom ( input: GenerateRandomRequest ) returns  ( output: Result<GenerateRandomResponse, Error> )
+ predicate {:opaque} GenerateRandomCalledWith ( input: GenerateRandomRequest ) {true}
+ predicate {:opaque} GenerateRandomSucceededWith (  input: GenerateRandomRequest , output: GenerateRandomResponse ) {true}
+ method GenerateRandom ( input: GenerateRandomRequest ) returns (output: Result<GenerateRandomResponse, Error>)
 	ensures GenerateRandomCalledWith (  input )
 	ensures output.Success? ==> GenerateRandomSucceededWith (  input , output.value )
 
- predicate GetKeyPolicyCalledWith ( input: GetKeyPolicyRequest ) {true}
- predicate GetKeyPolicySucceededWith (  input: GetKeyPolicyRequest , output: GetKeyPolicyResponse ) {true}
- method GetKeyPolicy ( input: GetKeyPolicyRequest ) returns  ( output: Result<GetKeyPolicyResponse, Error> )
+ predicate {:opaque} GetKeyPolicyCalledWith ( input: GetKeyPolicyRequest ) {true}
+ predicate {:opaque} GetKeyPolicySucceededWith (  input: GetKeyPolicyRequest , output: GetKeyPolicyResponse ) {true}
+ method GetKeyPolicy ( input: GetKeyPolicyRequest ) returns (output: Result<GetKeyPolicyResponse, Error>)
 	ensures GetKeyPolicyCalledWith (  input )
 	ensures output.Success? ==> GetKeyPolicySucceededWith (  input , output.value )
 
- predicate GetKeyRotationStatusCalledWith ( input: GetKeyRotationStatusRequest ) {true}
- predicate GetKeyRotationStatusSucceededWith (  input: GetKeyRotationStatusRequest , output: GetKeyRotationStatusResponse ) {true}
- method GetKeyRotationStatus ( input: GetKeyRotationStatusRequest ) returns  ( output: Result<GetKeyRotationStatusResponse, Error> )
+ predicate {:opaque} GetKeyRotationStatusCalledWith ( input: GetKeyRotationStatusRequest ) {true}
+ predicate {:opaque} GetKeyRotationStatusSucceededWith (  input: GetKeyRotationStatusRequest , output: GetKeyRotationStatusResponse ) {true}
+ method GetKeyRotationStatus ( input: GetKeyRotationStatusRequest ) returns (output: Result<GetKeyRotationStatusResponse, Error>)
 	ensures GetKeyRotationStatusCalledWith (  input )
 	ensures output.Success? ==> GetKeyRotationStatusSucceededWith (  input , output.value )
 
- predicate GetParametersForImportCalledWith ( input: GetParametersForImportRequest ) {true}
- predicate GetParametersForImportSucceededWith (  input: GetParametersForImportRequest , output: GetParametersForImportResponse ) {true}
- method GetParametersForImport ( input: GetParametersForImportRequest ) returns  ( output: Result<GetParametersForImportResponse, Error> )
+ predicate {:opaque} GetParametersForImportCalledWith ( input: GetParametersForImportRequest ) {true}
+ predicate {:opaque} GetParametersForImportSucceededWith (  input: GetParametersForImportRequest , output: GetParametersForImportResponse ) {true}
+ method GetParametersForImport ( input: GetParametersForImportRequest ) returns (output: Result<GetParametersForImportResponse, Error>)
 	ensures GetParametersForImportCalledWith (  input )
 	ensures output.Success? ==> GetParametersForImportSucceededWith (  input , output.value )
 
- predicate GetPublicKeyCalledWith ( input: GetPublicKeyRequest ) {true}
- predicate GetPublicKeySucceededWith (  input: GetPublicKeyRequest , output: GetPublicKeyResponse ) {true}
- method GetPublicKey ( input: GetPublicKeyRequest ) returns  ( output: Result<GetPublicKeyResponse, Error> )
+ predicate {:opaque} GetPublicKeyCalledWith ( input: GetPublicKeyRequest ) {true}
+ predicate {:opaque} GetPublicKeySucceededWith (  input: GetPublicKeyRequest , output: GetPublicKeyResponse ) {true}
+ method GetPublicKey ( input: GetPublicKeyRequest ) returns (output: Result<GetPublicKeyResponse, Error>)
 	ensures GetPublicKeyCalledWith (  input )
 	ensures output.Success? ==> GetPublicKeySucceededWith (  input , output.value )
 
- predicate ImportKeyMaterialCalledWith ( input: ImportKeyMaterialRequest ) {true}
- predicate ImportKeyMaterialSucceededWith (  input: ImportKeyMaterialRequest , output: ImportKeyMaterialResponse ) {true}
- method ImportKeyMaterial ( input: ImportKeyMaterialRequest ) returns  ( output: Result<ImportKeyMaterialResponse, Error> )
+ predicate {:opaque} ImportKeyMaterialCalledWith ( input: ImportKeyMaterialRequest ) {true}
+ predicate {:opaque} ImportKeyMaterialSucceededWith (  input: ImportKeyMaterialRequest , output: ImportKeyMaterialResponse ) {true}
+ method ImportKeyMaterial ( input: ImportKeyMaterialRequest ) returns (output: Result<ImportKeyMaterialResponse, Error>)
 	ensures ImportKeyMaterialCalledWith (  input )
 	ensures output.Success? ==> ImportKeyMaterialSucceededWith (  input , output.value )
 
- predicate ListAliasesCalledWith ( input: ListAliasesRequest ) {true}
- predicate ListAliasesSucceededWith (  input: ListAliasesRequest , output: ListAliasesResponse ) {true}
- method ListAliases ( input: ListAliasesRequest ) returns  ( output: Result<ListAliasesResponse, Error> )
+ predicate {:opaque} ListAliasesCalledWith ( input: ListAliasesRequest ) {true}
+ predicate {:opaque} ListAliasesSucceededWith (  input: ListAliasesRequest , output: ListAliasesResponse ) {true}
+ method ListAliases ( input: ListAliasesRequest ) returns (output: Result<ListAliasesResponse, Error>)
 	ensures ListAliasesCalledWith (  input )
 	ensures output.Success? ==> ListAliasesSucceededWith (  input , output.value )
 
- predicate ListGrantsCalledWith ( input: ListGrantsRequest ) {true}
- predicate ListGrantsSucceededWith (  input: ListGrantsRequest , output: ListGrantsResponse ) {true}
- method ListGrants ( input: ListGrantsRequest ) returns  ( output: Result<ListGrantsResponse, Error> )
+ predicate {:opaque} ListGrantsCalledWith ( input: ListGrantsRequest ) {true}
+ predicate {:opaque} ListGrantsSucceededWith (  input: ListGrantsRequest , output: ListGrantsResponse ) {true}
+ method ListGrants ( input: ListGrantsRequest ) returns (output: Result<ListGrantsResponse, Error>)
 	ensures ListGrantsCalledWith (  input )
 	ensures output.Success? ==> ListGrantsSucceededWith (  input , output.value )
 
- predicate ListKeyPoliciesCalledWith ( input: ListKeyPoliciesRequest ) {true}
- predicate ListKeyPoliciesSucceededWith (  input: ListKeyPoliciesRequest , output: ListKeyPoliciesResponse ) {true}
- method ListKeyPolicies ( input: ListKeyPoliciesRequest ) returns  ( output: Result<ListKeyPoliciesResponse, Error> )
+ predicate {:opaque} ListKeyPoliciesCalledWith ( input: ListKeyPoliciesRequest ) {true}
+ predicate {:opaque} ListKeyPoliciesSucceededWith (  input: ListKeyPoliciesRequest , output: ListKeyPoliciesResponse ) {true}
+ method ListKeyPolicies ( input: ListKeyPoliciesRequest ) returns (output: Result<ListKeyPoliciesResponse, Error>)
 	ensures ListKeyPoliciesCalledWith (  input )
 	ensures output.Success? ==> ListKeyPoliciesSucceededWith (  input , output.value )
 
- predicate ListResourceTagsCalledWith ( input: ListResourceTagsRequest ) {true}
- predicate ListResourceTagsSucceededWith (  input: ListResourceTagsRequest , output: ListResourceTagsResponse ) {true}
- method ListResourceTags ( input: ListResourceTagsRequest ) returns  ( output: Result<ListResourceTagsResponse, Error> )
+ predicate {:opaque} ListResourceTagsCalledWith ( input: ListResourceTagsRequest ) {true}
+ predicate {:opaque} ListResourceTagsSucceededWith (  input: ListResourceTagsRequest , output: ListResourceTagsResponse ) {true}
+ method ListResourceTags ( input: ListResourceTagsRequest ) returns (output: Result<ListResourceTagsResponse, Error>)
 	ensures ListResourceTagsCalledWith (  input )
 	ensures output.Success? ==> ListResourceTagsSucceededWith (  input , output.value )
 
- predicate PutKeyPolicyCalledWith ( input: PutKeyPolicyRequest ) {true}
- predicate PutKeyPolicySucceededWith (  input: PutKeyPolicyRequest ) {true}
- method PutKeyPolicy ( input: PutKeyPolicyRequest ) returns  ( output: Result<(), Error> )
+ predicate {:opaque} PutKeyPolicyCalledWith ( input: PutKeyPolicyRequest ) {true}
+ predicate {:opaque} PutKeyPolicySucceededWith (  input: PutKeyPolicyRequest ) {true}
+ method PutKeyPolicy ( input: PutKeyPolicyRequest ) returns (output: Result<(), Error>)
 	ensures PutKeyPolicyCalledWith (  input )
 	ensures output.Success? ==> PutKeyPolicySucceededWith (  input )
 
- predicate ReEncryptCalledWith ( input: ReEncryptRequest ) {true}
- predicate ReEncryptSucceededWith (  input: ReEncryptRequest , output: ReEncryptResponse ) {true}
- method ReEncrypt ( input: ReEncryptRequest ) returns  ( output: Result<ReEncryptResponse, Error> )
+ predicate {:opaque} ReEncryptCalledWith ( input: ReEncryptRequest ) {true}
+ predicate {:opaque} ReEncryptSucceededWith (  input: ReEncryptRequest , output: ReEncryptResponse ) {true}
+ method ReEncrypt ( input: ReEncryptRequest ) returns (output: Result<ReEncryptResponse, Error>)
 	ensures ReEncryptCalledWith (  input )
 	ensures output.Success? ==> ReEncryptSucceededWith (  input , output.value )
 
- predicate ReplicateKeyCalledWith ( input: ReplicateKeyRequest ) {true}
- predicate ReplicateKeySucceededWith (  input: ReplicateKeyRequest , output: ReplicateKeyResponse ) {true}
- method ReplicateKey ( input: ReplicateKeyRequest ) returns  ( output: Result<ReplicateKeyResponse, Error> )
+ predicate {:opaque} ReplicateKeyCalledWith ( input: ReplicateKeyRequest ) {true}
+ predicate {:opaque} ReplicateKeySucceededWith (  input: ReplicateKeyRequest , output: ReplicateKeyResponse ) {true}
+ method ReplicateKey ( input: ReplicateKeyRequest ) returns (output: Result<ReplicateKeyResponse, Error>)
 	ensures ReplicateKeyCalledWith (  input )
 	ensures output.Success? ==> ReplicateKeySucceededWith (  input , output.value )
 
- predicate RetireGrantCalledWith ( input: RetireGrantRequest ) {true}
- predicate RetireGrantSucceededWith (  input: RetireGrantRequest ) {true}
- method RetireGrant ( input: RetireGrantRequest ) returns  ( output: Result<(), Error> )
+ predicate {:opaque} RetireGrantCalledWith ( input: RetireGrantRequest ) {true}
+ predicate {:opaque} RetireGrantSucceededWith (  input: RetireGrantRequest ) {true}
+ method RetireGrant ( input: RetireGrantRequest ) returns (output: Result<(), Error>)
 	ensures RetireGrantCalledWith (  input )
 	ensures output.Success? ==> RetireGrantSucceededWith (  input )
 
- predicate RevokeGrantCalledWith ( input: RevokeGrantRequest ) {true}
- predicate RevokeGrantSucceededWith (  input: RevokeGrantRequest ) {true}
- method RevokeGrant ( input: RevokeGrantRequest ) returns  ( output: Result<(), Error> )
+ predicate {:opaque} RevokeGrantCalledWith ( input: RevokeGrantRequest ) {true}
+ predicate {:opaque} RevokeGrantSucceededWith (  input: RevokeGrantRequest ) {true}
+ method RevokeGrant ( input: RevokeGrantRequest ) returns (output: Result<(), Error>)
 	ensures RevokeGrantCalledWith (  input )
 	ensures output.Success? ==> RevokeGrantSucceededWith (  input )
 
- predicate ScheduleKeyDeletionCalledWith ( input: ScheduleKeyDeletionRequest ) {true}
- predicate ScheduleKeyDeletionSucceededWith (  input: ScheduleKeyDeletionRequest , output: ScheduleKeyDeletionResponse ) {true}
- method ScheduleKeyDeletion ( input: ScheduleKeyDeletionRequest ) returns  ( output: Result<ScheduleKeyDeletionResponse, Error> )
+ predicate {:opaque} ScheduleKeyDeletionCalledWith ( input: ScheduleKeyDeletionRequest ) {true}
+ predicate {:opaque} ScheduleKeyDeletionSucceededWith (  input: ScheduleKeyDeletionRequest , output: ScheduleKeyDeletionResponse ) {true}
+ method ScheduleKeyDeletion ( input: ScheduleKeyDeletionRequest ) returns (output: Result<ScheduleKeyDeletionResponse, Error>)
 	ensures ScheduleKeyDeletionCalledWith (  input )
 	ensures output.Success? ==> ScheduleKeyDeletionSucceededWith (  input , output.value )
 
- predicate SignCalledWith ( input: SignRequest ) {true}
- predicate SignSucceededWith (  input: SignRequest , output: SignResponse ) {true}
- method Sign ( input: SignRequest ) returns  ( output: Result<SignResponse, Error> )
+ predicate {:opaque} SignCalledWith ( input: SignRequest ) {true}
+ predicate {:opaque} SignSucceededWith (  input: SignRequest , output: SignResponse ) {true}
+ method Sign ( input: SignRequest ) returns (output: Result<SignResponse, Error>)
 	ensures SignCalledWith (  input )
 	ensures output.Success? ==> SignSucceededWith (  input , output.value )
 
- predicate TagResourceCalledWith ( input: TagResourceRequest ) {true}
- predicate TagResourceSucceededWith (  input: TagResourceRequest ) {true}
- method TagResource ( input: TagResourceRequest ) returns  ( output: Result<(), Error> )
+ predicate {:opaque} TagResourceCalledWith ( input: TagResourceRequest ) {true}
+ predicate {:opaque} TagResourceSucceededWith (  input: TagResourceRequest ) {true}
+ method TagResource ( input: TagResourceRequest ) returns (output: Result<(), Error>)
 	ensures TagResourceCalledWith (  input )
 	ensures output.Success? ==> TagResourceSucceededWith (  input )
 
- predicate UntagResourceCalledWith ( input: UntagResourceRequest ) {true}
- predicate UntagResourceSucceededWith (  input: UntagResourceRequest ) {true}
- method UntagResource ( input: UntagResourceRequest ) returns  ( output: Result<(), Error> )
+ predicate {:opaque} UntagResourceCalledWith ( input: UntagResourceRequest ) {true}
+ predicate {:opaque} UntagResourceSucceededWith (  input: UntagResourceRequest ) {true}
+ method UntagResource ( input: UntagResourceRequest ) returns (output: Result<(), Error>)
 	ensures UntagResourceCalledWith (  input )
 	ensures output.Success? ==> UntagResourceSucceededWith (  input )
 
- predicate UpdateAliasCalledWith ( input: UpdateAliasRequest ) {true}
- predicate UpdateAliasSucceededWith (  input: UpdateAliasRequest ) {true}
- method UpdateAlias ( input: UpdateAliasRequest ) returns  ( output: Result<(), Error> )
+ predicate {:opaque} UpdateAliasCalledWith ( input: UpdateAliasRequest ) {true}
+ predicate {:opaque} UpdateAliasSucceededWith (  input: UpdateAliasRequest ) {true}
+ method UpdateAlias ( input: UpdateAliasRequest ) returns (output: Result<(), Error>)
 	ensures UpdateAliasCalledWith (  input )
 	ensures output.Success? ==> UpdateAliasSucceededWith (  input )
 
- predicate UpdateCustomKeyStoreCalledWith ( input: UpdateCustomKeyStoreRequest ) {true}
- predicate UpdateCustomKeyStoreSucceededWith (  input: UpdateCustomKeyStoreRequest , output: UpdateCustomKeyStoreResponse ) {true}
- method UpdateCustomKeyStore ( input: UpdateCustomKeyStoreRequest ) returns  ( output: Result<UpdateCustomKeyStoreResponse, Error> )
+ predicate {:opaque} UpdateCustomKeyStoreCalledWith ( input: UpdateCustomKeyStoreRequest ) {true}
+ predicate {:opaque} UpdateCustomKeyStoreSucceededWith (  input: UpdateCustomKeyStoreRequest , output: UpdateCustomKeyStoreResponse ) {true}
+ method UpdateCustomKeyStore ( input: UpdateCustomKeyStoreRequest ) returns (output: Result<UpdateCustomKeyStoreResponse, Error>)
 	ensures UpdateCustomKeyStoreCalledWith (  input )
 	ensures output.Success? ==> UpdateCustomKeyStoreSucceededWith (  input , output.value )
 
- predicate UpdateKeyDescriptionCalledWith ( input: UpdateKeyDescriptionRequest ) {true}
- predicate UpdateKeyDescriptionSucceededWith (  input: UpdateKeyDescriptionRequest ) {true}
- method UpdateKeyDescription ( input: UpdateKeyDescriptionRequest ) returns  ( output: Result<(), Error> )
+ predicate {:opaque} UpdateKeyDescriptionCalledWith ( input: UpdateKeyDescriptionRequest ) {true}
+ predicate {:opaque} UpdateKeyDescriptionSucceededWith (  input: UpdateKeyDescriptionRequest ) {true}
+ method UpdateKeyDescription ( input: UpdateKeyDescriptionRequest ) returns (output: Result<(), Error>)
 	ensures UpdateKeyDescriptionCalledWith (  input )
 	ensures output.Success? ==> UpdateKeyDescriptionSucceededWith (  input )
 
- predicate UpdatePrimaryRegionCalledWith ( input: UpdatePrimaryRegionRequest ) {true}
- predicate UpdatePrimaryRegionSucceededWith (  input: UpdatePrimaryRegionRequest ) {true}
- method UpdatePrimaryRegion ( input: UpdatePrimaryRegionRequest ) returns  ( output: Result<(), Error> )
+ predicate {:opaque} UpdatePrimaryRegionCalledWith ( input: UpdatePrimaryRegionRequest ) {true}
+ predicate {:opaque} UpdatePrimaryRegionSucceededWith (  input: UpdatePrimaryRegionRequest ) {true}
+ method UpdatePrimaryRegion ( input: UpdatePrimaryRegionRequest ) returns (output: Result<(), Error>)
 	ensures UpdatePrimaryRegionCalledWith (  input )
 	ensures output.Success? ==> UpdatePrimaryRegionSucceededWith (  input )
 
- predicate VerifyCalledWith ( input: VerifyRequest ) {true}
- predicate VerifySucceededWith (  input: VerifyRequest , output: VerifyResponse ) {true}
- method Verify ( input: VerifyRequest ) returns  ( output: Result<VerifyResponse, Error> )
+ predicate {:opaque} VerifyCalledWith ( input: VerifyRequest ) {true}
+ predicate {:opaque} VerifySucceededWith (  input: VerifyRequest , output: VerifyResponse ) {true}
+ method Verify ( input: VerifyRequest ) returns (output: Result<VerifyResponse, Error>)
 	ensures VerifyCalledWith (  input )
 	ensures output.Success? ==> VerifySucceededWith (  input , output.value )
 
@@ -565,7 +673,8 @@ include "../../StandardLibrary/StandardLibrary.dfy"
  datatype KeyManagerType =
 	| AWS
 	| CUSTOMER
- datatype KeyMetadata = KeyMetadata ( nameonly AWSAccountId: Option<AWSAccountIdType> ,
+ datatype KeyMetadata = | KeyMetadata (
+ nameonly AWSAccountId: Option<AWSAccountIdType> ,
  nameonly KeyId: KeyIdType ,
  nameonly Arn: Option<ArnType> ,
  nameonly CreationDate: Option<string> ,
@@ -586,7 +695,8 @@ include "../../StandardLibrary/StandardLibrary.dfy"
  nameonly SigningAlgorithms: Option<SigningAlgorithmSpecList> ,
  nameonly MultiRegion: Option<NullableBooleanType> ,
  nameonly MultiRegionConfiguration: Option<MultiRegionConfiguration> ,
- nameonly PendingDeletionWindowInDays: Option<PendingWindowInDaysType> )
+ nameonly PendingDeletionWindowInDays: Option<PendingWindowInDaysType>
+ )
  datatype KeySpec =
 	| RSA_2048
 	| RSA_3072
@@ -616,37 +726,57 @@ include "../../StandardLibrary/StandardLibrary.dfy"
  predicate method IsValid_LimitType(x: int32) {
  ( 1 <= x <= 1000 )
 }
- datatype ListAliasesRequest = ListAliasesRequest ( nameonly KeyId: Option<KeyIdType> ,
+ datatype ListAliasesRequest = | ListAliasesRequest (
+ nameonly KeyId: Option<KeyIdType> ,
  nameonly Limit: Option<LimitType> ,
- nameonly Marker: Option<MarkerType> )
- datatype ListAliasesResponse = ListAliasesResponse ( nameonly Aliases: Option<AliasList> ,
+ nameonly Marker: Option<MarkerType>
+ )
+ datatype ListAliasesResponse = | ListAliasesResponse (
+ nameonly Aliases: Option<AliasList> ,
  nameonly NextMarker: Option<MarkerType> ,
- nameonly Truncated: Option<BooleanType> )
- datatype ListGrantsRequest = ListGrantsRequest ( nameonly Limit: Option<LimitType> ,
+ nameonly Truncated: Option<BooleanType>
+ )
+ datatype ListGrantsRequest = | ListGrantsRequest (
+ nameonly Limit: Option<LimitType> ,
  nameonly Marker: Option<MarkerType> ,
  nameonly KeyId: KeyIdType ,
  nameonly GrantId: Option<GrantIdType> ,
- nameonly GranteePrincipal: Option<PrincipalIdType> )
- datatype ListGrantsResponse = ListGrantsResponse ( nameonly Grants: Option<GrantList> ,
+ nameonly GranteePrincipal: Option<PrincipalIdType>
+ )
+ datatype ListGrantsResponse = | ListGrantsResponse (
+ nameonly Grants: Option<GrantList> ,
  nameonly NextMarker: Option<MarkerType> ,
- nameonly Truncated: Option<BooleanType> )
- datatype ListKeyPoliciesRequest = ListKeyPoliciesRequest ( nameonly KeyId: KeyIdType ,
+ nameonly Truncated: Option<BooleanType>
+ )
+ datatype ListKeyPoliciesRequest = | ListKeyPoliciesRequest (
+ nameonly KeyId: KeyIdType ,
  nameonly Limit: Option<LimitType> ,
- nameonly Marker: Option<MarkerType> )
- datatype ListKeyPoliciesResponse = ListKeyPoliciesResponse ( nameonly PolicyNames: Option<PolicyNameList> ,
+ nameonly Marker: Option<MarkerType>
+ )
+ datatype ListKeyPoliciesResponse = | ListKeyPoliciesResponse (
+ nameonly PolicyNames: Option<PolicyNameList> ,
  nameonly NextMarker: Option<MarkerType> ,
- nameonly Truncated: Option<BooleanType> )
- datatype ListKeysRequest = ListKeysRequest ( nameonly Limit: Option<LimitType> ,
- nameonly Marker: Option<MarkerType> )
- datatype ListResourceTagsRequest = ListResourceTagsRequest ( nameonly KeyId: KeyIdType ,
+ nameonly Truncated: Option<BooleanType>
+ )
+ datatype ListKeysRequest = | ListKeysRequest (
  nameonly Limit: Option<LimitType> ,
- nameonly Marker: Option<MarkerType> )
- datatype ListResourceTagsResponse = ListResourceTagsResponse ( nameonly Tags: Option<TagList> ,
+ nameonly Marker: Option<MarkerType>
+ )
+ datatype ListResourceTagsRequest = | ListResourceTagsRequest (
+ nameonly KeyId: KeyIdType ,
+ nameonly Limit: Option<LimitType> ,
+ nameonly Marker: Option<MarkerType>
+ )
+ datatype ListResourceTagsResponse = | ListResourceTagsResponse (
+ nameonly Tags: Option<TagList> ,
  nameonly NextMarker: Option<MarkerType> ,
- nameonly Truncated: Option<BooleanType> )
- datatype ListRetirableGrantsRequest = ListRetirableGrantsRequest ( nameonly Limit: Option<LimitType> ,
+ nameonly Truncated: Option<BooleanType>
+ )
+ datatype ListRetirableGrantsRequest = | ListRetirableGrantsRequest (
+ nameonly Limit: Option<LimitType> ,
  nameonly Marker: Option<MarkerType> ,
- nameonly RetiringPrincipal: PrincipalIdType )
+ nameonly RetiringPrincipal: PrincipalIdType
+ )
  type MarkerType = x: string | IsValid_MarkerType(x) witness *
  predicate method IsValid_MarkerType(x: string) {
  ( 1 <= |x| <= 1024 )
@@ -654,11 +784,15 @@ include "../../StandardLibrary/StandardLibrary.dfy"
  datatype MessageType =
 	| RAW
 	| DIGEST
- datatype MultiRegionConfiguration = MultiRegionConfiguration ( nameonly MultiRegionKeyType: Option<MultiRegionKeyType> ,
+ datatype MultiRegionConfiguration = | MultiRegionConfiguration (
+ nameonly MultiRegionKeyType: Option<MultiRegionKeyType> ,
  nameonly PrimaryKey: Option<MultiRegionKey> ,
- nameonly ReplicaKeys: Option<MultiRegionKeyList> )
- datatype MultiRegionKey = MultiRegionKey ( nameonly Arn: Option<ArnType> ,
- nameonly Region: Option<RegionType> )
+ nameonly ReplicaKeys: Option<MultiRegionKeyList>
+ )
+ datatype MultiRegionKey = | MultiRegionKey (
+ nameonly Arn: Option<ArnType> ,
+ nameonly Region: Option<RegionType>
+ )
  type MultiRegionKeyList = seq<MultiRegionKey>
  datatype MultiRegionKeyType =
 	| PRIMARY
@@ -697,47 +831,65 @@ include "../../StandardLibrary/StandardLibrary.dfy"
  predicate method IsValid_PublicKeyType(x: seq<uint8>) {
  ( 1 <= |x| <= 8192 )
 }
- datatype PutKeyPolicyRequest = PutKeyPolicyRequest ( nameonly KeyId: KeyIdType ,
+ datatype PutKeyPolicyRequest = | PutKeyPolicyRequest (
+ nameonly KeyId: KeyIdType ,
  nameonly PolicyName: PolicyNameType ,
  nameonly Policy: PolicyType ,
- nameonly BypassPolicyLockoutSafetyCheck: Option<BooleanType> )
- datatype ReEncryptRequest = ReEncryptRequest ( nameonly CiphertextBlob: CiphertextType ,
+ nameonly BypassPolicyLockoutSafetyCheck: Option<BooleanType>
+ )
+ datatype ReEncryptRequest = | ReEncryptRequest (
+ nameonly CiphertextBlob: CiphertextType ,
  nameonly SourceEncryptionContext: Option<EncryptionContextType> ,
  nameonly SourceKeyId: Option<KeyIdType> ,
  nameonly DestinationKeyId: KeyIdType ,
  nameonly DestinationEncryptionContext: Option<EncryptionContextType> ,
  nameonly SourceEncryptionAlgorithm: Option<EncryptionAlgorithmSpec> ,
  nameonly DestinationEncryptionAlgorithm: Option<EncryptionAlgorithmSpec> ,
- nameonly GrantTokens: Option<GrantTokenList> )
- datatype ReEncryptResponse = ReEncryptResponse ( nameonly CiphertextBlob: Option<CiphertextType> ,
+ nameonly GrantTokens: Option<GrantTokenList>
+ )
+ datatype ReEncryptResponse = | ReEncryptResponse (
+ nameonly CiphertextBlob: Option<CiphertextType> ,
  nameonly SourceKeyId: Option<KeyIdType> ,
  nameonly KeyId: Option<KeyIdType> ,
  nameonly SourceEncryptionAlgorithm: Option<EncryptionAlgorithmSpec> ,
- nameonly DestinationEncryptionAlgorithm: Option<EncryptionAlgorithmSpec> )
+ nameonly DestinationEncryptionAlgorithm: Option<EncryptionAlgorithmSpec>
+ )
  type RegionType = x: string | IsValid_RegionType(x) witness *
  predicate method IsValid_RegionType(x: string) {
  ( 1 <= |x| <= 32 )
 }
- datatype ReplicateKeyRequest = ReplicateKeyRequest ( nameonly KeyId: KeyIdType ,
+ datatype ReplicateKeyRequest = | ReplicateKeyRequest (
+ nameonly KeyId: KeyIdType ,
  nameonly ReplicaRegion: RegionType ,
  nameonly Policy: Option<PolicyType> ,
  nameonly BypassPolicyLockoutSafetyCheck: Option<BooleanType> ,
  nameonly Description: Option<DescriptionType> ,
- nameonly Tags: Option<TagList> )
- datatype ReplicateKeyResponse = ReplicateKeyResponse ( nameonly ReplicaKeyMetadata: Option<KeyMetadata> ,
+ nameonly Tags: Option<TagList>
+ )
+ datatype ReplicateKeyResponse = | ReplicateKeyResponse (
+ nameonly ReplicaKeyMetadata: Option<KeyMetadata> ,
  nameonly ReplicaPolicy: Option<PolicyType> ,
- nameonly ReplicaTags: Option<TagList> )
- datatype RetireGrantRequest = RetireGrantRequest ( nameonly GrantToken: Option<GrantTokenType> ,
+ nameonly ReplicaTags: Option<TagList>
+ )
+ datatype RetireGrantRequest = | RetireGrantRequest (
+ nameonly GrantToken: Option<GrantTokenType> ,
  nameonly KeyId: Option<KeyIdType> ,
- nameonly GrantId: Option<GrantIdType> )
- datatype RevokeGrantRequest = RevokeGrantRequest ( nameonly KeyId: KeyIdType ,
- nameonly GrantId: GrantIdType )
- datatype ScheduleKeyDeletionRequest = ScheduleKeyDeletionRequest ( nameonly KeyId: KeyIdType ,
- nameonly PendingWindowInDays: Option<PendingWindowInDaysType> )
- datatype ScheduleKeyDeletionResponse = ScheduleKeyDeletionResponse ( nameonly KeyId: Option<KeyIdType> ,
+ nameonly GrantId: Option<GrantIdType>
+ )
+ datatype RevokeGrantRequest = | RevokeGrantRequest (
+ nameonly KeyId: KeyIdType ,
+ nameonly GrantId: GrantIdType
+ )
+ datatype ScheduleKeyDeletionRequest = | ScheduleKeyDeletionRequest (
+ nameonly KeyId: KeyIdType ,
+ nameonly PendingWindowInDays: Option<PendingWindowInDaysType>
+ )
+ datatype ScheduleKeyDeletionResponse = | ScheduleKeyDeletionResponse (
+ nameonly KeyId: Option<KeyIdType> ,
  nameonly DeletionDate: Option<string> ,
  nameonly KeyState: Option<KeyState> ,
- nameonly PendingWindowInDays: Option<PendingWindowInDaysType> )
+ nameonly PendingWindowInDays: Option<PendingWindowInDaysType>
+ )
  datatype SigningAlgorithmSpec =
 	| RSASSA_PSS_SHA_256
 	| RSASSA_PSS_SHA_384
@@ -749,24 +901,32 @@ include "../../StandardLibrary/StandardLibrary.dfy"
 	| ECDSA_SHA_384
 	| ECDSA_SHA_512
  type SigningAlgorithmSpecList = seq<SigningAlgorithmSpec>
- datatype SignRequest = SignRequest ( nameonly KeyId: KeyIdType ,
+ datatype SignRequest = | SignRequest (
+ nameonly KeyId: KeyIdType ,
  nameonly Message: PlaintextType ,
  nameonly MessageType: Option<MessageType> ,
  nameonly GrantTokens: Option<GrantTokenList> ,
- nameonly SigningAlgorithm: SigningAlgorithmSpec )
- datatype SignResponse = SignResponse ( nameonly KeyId: Option<KeyIdType> ,
+ nameonly SigningAlgorithm: SigningAlgorithmSpec
+ )
+ datatype SignResponse = | SignResponse (
+ nameonly KeyId: Option<KeyIdType> ,
  nameonly Signature: Option<CiphertextType> ,
- nameonly SigningAlgorithm: Option<SigningAlgorithmSpec> )
- datatype Tag = Tag ( nameonly TagKey: TagKeyType ,
- nameonly TagValue: TagValueType )
+ nameonly SigningAlgorithm: Option<SigningAlgorithmSpec>
+ )
+ datatype Tag = | Tag (
+ nameonly TagKey: TagKeyType ,
+ nameonly TagValue: TagValueType
+ )
  type TagKeyList = seq<TagKeyType>
  type TagKeyType = x: string | IsValid_TagKeyType(x) witness *
  predicate method IsValid_TagKeyType(x: string) {
  ( 1 <= |x| <= 128 )
 }
  type TagList = seq<Tag>
- datatype TagResourceRequest = TagResourceRequest ( nameonly KeyId: KeyIdType ,
- nameonly Tags: TagList )
+ datatype TagResourceRequest = | TagResourceRequest (
+ nameonly KeyId: KeyIdType ,
+ nameonly Tags: TagList
+ )
  type TagValueType = x: string | IsValid_TagValueType(x) witness *
  predicate method IsValid_TagValueType(x: string) {
  ( 0 <= |x| <= 256 )
@@ -775,68 +935,304 @@ include "../../StandardLibrary/StandardLibrary.dfy"
  predicate method IsValid_TrustAnchorCertificateType(x: string) {
  ( 1 <= |x| <= 5000 )
 }
- datatype UntagResourceRequest = UntagResourceRequest ( nameonly KeyId: KeyIdType ,
- nameonly TagKeys: TagKeyList )
- datatype UpdateAliasRequest = UpdateAliasRequest ( nameonly AliasName: AliasNameType ,
- nameonly TargetKeyId: KeyIdType )
- datatype UpdateCustomKeyStoreRequest = UpdateCustomKeyStoreRequest ( nameonly CustomKeyStoreId: CustomKeyStoreIdType ,
+ datatype UntagResourceRequest = | UntagResourceRequest (
+ nameonly KeyId: KeyIdType ,
+ nameonly TagKeys: TagKeyList
+ )
+ datatype UpdateAliasRequest = | UpdateAliasRequest (
+ nameonly AliasName: AliasNameType ,
+ nameonly TargetKeyId: KeyIdType
+ )
+ datatype UpdateCustomKeyStoreRequest = | UpdateCustomKeyStoreRequest (
+ nameonly CustomKeyStoreId: CustomKeyStoreIdType ,
  nameonly NewCustomKeyStoreName: Option<CustomKeyStoreNameType> ,
  nameonly KeyStorePassword: Option<KeyStorePasswordType> ,
- nameonly CloudHsmClusterId: Option<CloudHsmClusterIdType> )
- datatype UpdateCustomKeyStoreResponse = UpdateCustomKeyStoreResponse (  )
- datatype UpdateKeyDescriptionRequest = UpdateKeyDescriptionRequest ( nameonly KeyId: KeyIdType ,
- nameonly Description: DescriptionType )
- datatype UpdatePrimaryRegionRequest = UpdatePrimaryRegionRequest ( nameonly KeyId: KeyIdType ,
- nameonly PrimaryRegion: RegionType )
- datatype VerifyRequest = VerifyRequest ( nameonly KeyId: KeyIdType ,
+ nameonly CloudHsmClusterId: Option<CloudHsmClusterIdType>
+ )
+ datatype UpdateCustomKeyStoreResponse = | UpdateCustomKeyStoreResponse (
+ 
+ )
+ datatype UpdateKeyDescriptionRequest = | UpdateKeyDescriptionRequest (
+ nameonly KeyId: KeyIdType ,
+ nameonly Description: DescriptionType
+ )
+ datatype UpdatePrimaryRegionRequest = | UpdatePrimaryRegionRequest (
+ nameonly KeyId: KeyIdType ,
+ nameonly PrimaryRegion: RegionType
+ )
+ datatype VerifyRequest = | VerifyRequest (
+ nameonly KeyId: KeyIdType ,
  nameonly Message: PlaintextType ,
  nameonly MessageType: Option<MessageType> ,
  nameonly Signature: CiphertextType ,
  nameonly SigningAlgorithm: SigningAlgorithmSpec ,
- nameonly GrantTokens: Option<GrantTokenList> )
- datatype VerifyResponse = VerifyResponse ( nameonly KeyId: Option<KeyIdType> ,
+ nameonly GrantTokens: Option<GrantTokenList>
+ )
+ datatype VerifyResponse = | VerifyResponse (
+ nameonly KeyId: Option<KeyIdType> ,
  nameonly SignatureValid: Option<BooleanType> ,
- nameonly SigningAlgorithm: Option<SigningAlgorithmSpec> )
+ nameonly SigningAlgorithm: Option<SigningAlgorithmSpec>
+ )
  datatype WrappingKeySpec =
 	| RSA_2048
  datatype Error =
  // Local Error structures are listed here
- | KeyUnavailableException ( nameonly message: Option<ErrorMessageType> )
- | KMSInvalidSignatureException ( nameonly message: Option<ErrorMessageType> )
- | KMSInternalException ( nameonly message: Option<ErrorMessageType> )
- | CustomKeyStoreInvalidStateException ( nameonly message: Option<ErrorMessageType> )
- | KMSInvalidStateException ( nameonly message: Option<ErrorMessageType> )
- | IncorrectTrustAnchorException ( nameonly message: Option<ErrorMessageType> )
- | ExpiredImportTokenException ( nameonly message: Option<ErrorMessageType> )
- | IncorrectKeyException ( nameonly message: Option<ErrorMessageType> )
- | CustomKeyStoreNameInUseException ( nameonly message: Option<ErrorMessageType> )
- | DisabledException ( nameonly message: Option<ErrorMessageType> )
- | InvalidArnException ( nameonly message: Option<ErrorMessageType> )
- | CloudHsmClusterInUseException ( nameonly message: Option<ErrorMessageType> )
- | InvalidKeyUsageException ( nameonly message: Option<ErrorMessageType> )
- | CloudHsmClusterNotFoundException ( nameonly message: Option<ErrorMessageType> )
- | CloudHsmClusterInvalidConfigurationException ( nameonly message: Option<ErrorMessageType> )
- | AlreadyExistsException ( nameonly message: Option<ErrorMessageType> )
- | TagException ( nameonly message: Option<ErrorMessageType> )
- | InvalidGrantIdException ( nameonly message: Option<ErrorMessageType> )
- | LimitExceededException ( nameonly message: Option<ErrorMessageType> )
- | InvalidMarkerException ( nameonly message: Option<ErrorMessageType> )
- | InvalidGrantTokenException ( nameonly message: Option<ErrorMessageType> )
- | IncorrectKeyMaterialException ( nameonly message: Option<ErrorMessageType> )
- | CloudHsmClusterNotActiveException ( nameonly message: Option<ErrorMessageType> )
- | InvalidCiphertextException ( nameonly message: Option<ErrorMessageType> )
- | UnsupportedOperationException ( nameonly message: Option<ErrorMessageType> )
- | InvalidAliasNameException ( nameonly message: Option<ErrorMessageType> )
- | NotFoundException ( nameonly message: Option<ErrorMessageType> )
- | CloudHsmClusterNotRelatedException ( nameonly message: Option<ErrorMessageType> )
- | DependencyTimeoutException ( nameonly message: Option<ErrorMessageType> )
- | CustomKeyStoreHasCMKsException ( nameonly message: Option<ErrorMessageType> )
- | MalformedPolicyDocumentException ( nameonly message: Option<ErrorMessageType> )
- | CustomKeyStoreNotFoundException ( nameonly message: Option<ErrorMessageType> )
- | InvalidImportTokenException ( nameonly message: Option<ErrorMessageType> )
+ | InvalidGrantTokenException (
+ nameonly message: Option<ErrorMessageType>
+ )
+ | CloudHsmClusterNotActiveException (
+ nameonly message: Option<ErrorMessageType>
+ )
+ | IncorrectKeyMaterialException (
+ nameonly message: Option<ErrorMessageType>
+ )
+ | InvalidImportTokenException (
+ nameonly message: Option<ErrorMessageType>
+ )
+ | InvalidAliasNameException (
+ nameonly message: Option<ErrorMessageType>
+ )
+ | InvalidKeyUsageException (
+ nameonly message: Option<ErrorMessageType>
+ )
+ | CloudHsmClusterNotFoundException (
+ nameonly message: Option<ErrorMessageType>
+ )
+ | TagException (
+ nameonly message: Option<ErrorMessageType>
+ )
+ | CustomKeyStoreNotFoundException (
+ nameonly message: Option<ErrorMessageType>
+ )
+ | InvalidArnException (
+ nameonly message: Option<ErrorMessageType>
+ )
+ | CloudHsmClusterNotRelatedException (
+ nameonly message: Option<ErrorMessageType>
+ )
+ | NotFoundException (
+ nameonly message: Option<ErrorMessageType>
+ )
+ | CloudHsmClusterInvalidConfigurationException (
+ nameonly message: Option<ErrorMessageType>
+ )
+ | CustomKeyStoreNameInUseException (
+ nameonly message: Option<ErrorMessageType>
+ )
+ | UnsupportedOperationException (
+ nameonly message: Option<ErrorMessageType>
+ )
+ | DependencyTimeoutException (
+ nameonly message: Option<ErrorMessageType>
+ )
+ | CloudHsmClusterInUseException (
+ nameonly message: Option<ErrorMessageType>
+ )
+ | DisabledException (
+ nameonly message: Option<ErrorMessageType>
+ )
+ | KeyUnavailableException (
+ nameonly message: Option<ErrorMessageType>
+ )
+ | KMSInvalidSignatureException (
+ nameonly message: Option<ErrorMessageType>
+ )
+ | IncorrectKeyException (
+ nameonly message: Option<ErrorMessageType>
+ )
+ | CustomKeyStoreInvalidStateException (
+ nameonly message: Option<ErrorMessageType>
+ )
+ | ExpiredImportTokenException (
+ nameonly message: Option<ErrorMessageType>
+ )
+ | KMSInvalidStateException (
+ nameonly message: Option<ErrorMessageType>
+ )
+ | InvalidMarkerException (
+ nameonly message: Option<ErrorMessageType>
+ )
+ | InvalidGrantIdException (
+ nameonly message: Option<ErrorMessageType>
+ )
+ | AlreadyExistsException (
+ nameonly message: Option<ErrorMessageType>
+ )
+ | MalformedPolicyDocumentException (
+ nameonly message: Option<ErrorMessageType>
+ )
+ | LimitExceededException (
+ nameonly message: Option<ErrorMessageType>
+ )
+ | CustomKeyStoreHasCMKsException (
+ nameonly message: Option<ErrorMessageType>
+ )
+ | IncorrectTrustAnchorException (
+ nameonly message: Option<ErrorMessageType>
+ )
+ | InvalidCiphertextException (
+ nameonly message: Option<ErrorMessageType>
+ )
+ | KMSInternalException (
+ nameonly message: Option<ErrorMessageType>
+ )
  // Any dependent models are listed here
  
  // The Opaque error, used for native, extern, wrapped or unknown errors
  | Opaque(obj: object)
  type OpaqueError = e: Error | e.Opaque? witness *
+}
+ abstract module ComAmazonawsKmsAbstract
+ {
+ import opened Wrappers
+ import opened StandardLibrary.UInt
+ import opened UTF8
+ import opened Types = ComAmazonawsKmsTypes
+ datatype KMSClientConfigType = KMSClientConfigType
+ function method DefaultKMSClientConfigType(): KMSClientConfigType
+ class {:extern}  KMS extends IKeyManagementServiceClient
+ {
+ const config: KMSClientConfigType
+ constructor {:extern} Config (config: KMSClientConfigType)
+ constructor {:extern} Default()
+
+ method {:extern} CancelKeyDeletion ( input: CancelKeyDeletionRequest ) returns (output: Result<CancelKeyDeletionResponse, Error>)
+	ensures CancelKeyDeletionCalledWith (  input )
+	ensures output.Success? ==> CancelKeyDeletionSucceededWith (  input , output.value )
+ method {:extern} ConnectCustomKeyStore ( input: ConnectCustomKeyStoreRequest ) returns (output: Result<ConnectCustomKeyStoreResponse, Error>)
+	ensures ConnectCustomKeyStoreCalledWith (  input )
+	ensures output.Success? ==> ConnectCustomKeyStoreSucceededWith (  input , output.value )
+ method {:extern} CreateAlias ( input: CreateAliasRequest ) returns (output: Result<(), Error>)
+	ensures CreateAliasCalledWith (  input )
+	ensures output.Success? ==> CreateAliasSucceededWith (  input )
+ method {:extern} CreateCustomKeyStore ( input: CreateCustomKeyStoreRequest ) returns (output: Result<CreateCustomKeyStoreResponse, Error>)
+	ensures CreateCustomKeyStoreCalledWith (  input )
+	ensures output.Success? ==> CreateCustomKeyStoreSucceededWith (  input , output.value )
+ method {:extern} CreateGrant ( input: CreateGrantRequest ) returns (output: Result<CreateGrantResponse, Error>)
+	ensures CreateGrantCalledWith (  input )
+	ensures output.Success? ==> CreateGrantSucceededWith (  input , output.value )
+ method {:extern} CreateKey ( input: CreateKeyRequest ) returns (output: Result<CreateKeyResponse, Error>)
+	ensures CreateKeyCalledWith (  input )
+	ensures output.Success? ==> CreateKeySucceededWith (  input , output.value )
+ method {:extern} Decrypt ( input: DecryptRequest ) returns (output: Result<DecryptResponse, Error>)
+	ensures DecryptCalledWith (  input )
+	ensures output.Success? ==> DecryptSucceededWith (  input , output.value )
+ method {:extern} DeleteAlias ( input: DeleteAliasRequest ) returns (output: Result<(), Error>)
+	ensures DeleteAliasCalledWith (  input )
+	ensures output.Success? ==> DeleteAliasSucceededWith (  input )
+ method {:extern} DeleteCustomKeyStore ( input: DeleteCustomKeyStoreRequest ) returns (output: Result<DeleteCustomKeyStoreResponse, Error>)
+	ensures DeleteCustomKeyStoreCalledWith (  input )
+	ensures output.Success? ==> DeleteCustomKeyStoreSucceededWith (  input , output.value )
+ method {:extern} DeleteImportedKeyMaterial ( input: DeleteImportedKeyMaterialRequest ) returns (output: Result<(), Error>)
+	ensures DeleteImportedKeyMaterialCalledWith (  input )
+	ensures output.Success? ==> DeleteImportedKeyMaterialSucceededWith (  input )
+ method {:extern} DescribeCustomKeyStores ( input: DescribeCustomKeyStoresRequest ) returns (output: Result<DescribeCustomKeyStoresResponse, Error>)
+	ensures DescribeCustomKeyStoresCalledWith (  input )
+	ensures output.Success? ==> DescribeCustomKeyStoresSucceededWith (  input , output.value )
+ method {:extern} DescribeKey ( input: DescribeKeyRequest ) returns (output: Result<DescribeKeyResponse, Error>)
+	ensures DescribeKeyCalledWith (  input )
+	ensures output.Success? ==> DescribeKeySucceededWith (  input , output.value )
+ method {:extern} DisableKey ( input: DisableKeyRequest ) returns (output: Result<(), Error>)
+	ensures DisableKeyCalledWith (  input )
+	ensures output.Success? ==> DisableKeySucceededWith (  input )
+ method {:extern} DisableKeyRotation ( input: DisableKeyRotationRequest ) returns (output: Result<(), Error>)
+	ensures DisableKeyRotationCalledWith (  input )
+	ensures output.Success? ==> DisableKeyRotationSucceededWith (  input )
+ method {:extern} DisconnectCustomKeyStore ( input: DisconnectCustomKeyStoreRequest ) returns (output: Result<DisconnectCustomKeyStoreResponse, Error>)
+	ensures DisconnectCustomKeyStoreCalledWith (  input )
+	ensures output.Success? ==> DisconnectCustomKeyStoreSucceededWith (  input , output.value )
+ method {:extern} EnableKey ( input: EnableKeyRequest ) returns (output: Result<(), Error>)
+	ensures EnableKeyCalledWith (  input )
+	ensures output.Success? ==> EnableKeySucceededWith (  input )
+ method {:extern} EnableKeyRotation ( input: EnableKeyRotationRequest ) returns (output: Result<(), Error>)
+	ensures EnableKeyRotationCalledWith (  input )
+	ensures output.Success? ==> EnableKeyRotationSucceededWith (  input )
+ method {:extern} Encrypt ( input: EncryptRequest ) returns (output: Result<EncryptResponse, Error>)
+	ensures EncryptCalledWith (  input )
+	ensures output.Success? ==> EncryptSucceededWith (  input , output.value )
+ method {:extern} GenerateDataKey ( input: GenerateDataKeyRequest ) returns (output: Result<GenerateDataKeyResponse, Error>)
+	ensures GenerateDataKeyCalledWith (  input )
+	ensures output.Success? ==> GenerateDataKeySucceededWith (  input , output.value )
+ method {:extern} GenerateDataKeyPair ( input: GenerateDataKeyPairRequest ) returns (output: Result<GenerateDataKeyPairResponse, Error>)
+	ensures GenerateDataKeyPairCalledWith (  input )
+	ensures output.Success? ==> GenerateDataKeyPairSucceededWith (  input , output.value )
+ method {:extern} GenerateDataKeyPairWithoutPlaintext ( input: GenerateDataKeyPairWithoutPlaintextRequest ) returns (output: Result<GenerateDataKeyPairWithoutPlaintextResponse, Error>)
+	ensures GenerateDataKeyPairWithoutPlaintextCalledWith (  input )
+	ensures output.Success? ==> GenerateDataKeyPairWithoutPlaintextSucceededWith (  input , output.value )
+ method {:extern} GenerateDataKeyWithoutPlaintext ( input: GenerateDataKeyWithoutPlaintextRequest ) returns (output: Result<GenerateDataKeyWithoutPlaintextResponse, Error>)
+	ensures GenerateDataKeyWithoutPlaintextCalledWith (  input )
+	ensures output.Success? ==> GenerateDataKeyWithoutPlaintextSucceededWith (  input , output.value )
+ method {:extern} GenerateRandom ( input: GenerateRandomRequest ) returns (output: Result<GenerateRandomResponse, Error>)
+	ensures GenerateRandomCalledWith (  input )
+	ensures output.Success? ==> GenerateRandomSucceededWith (  input , output.value )
+ method {:extern} GetKeyPolicy ( input: GetKeyPolicyRequest ) returns (output: Result<GetKeyPolicyResponse, Error>)
+	ensures GetKeyPolicyCalledWith (  input )
+	ensures output.Success? ==> GetKeyPolicySucceededWith (  input , output.value )
+ method {:extern} GetKeyRotationStatus ( input: GetKeyRotationStatusRequest ) returns (output: Result<GetKeyRotationStatusResponse, Error>)
+	ensures GetKeyRotationStatusCalledWith (  input )
+	ensures output.Success? ==> GetKeyRotationStatusSucceededWith (  input , output.value )
+ method {:extern} GetParametersForImport ( input: GetParametersForImportRequest ) returns (output: Result<GetParametersForImportResponse, Error>)
+	ensures GetParametersForImportCalledWith (  input )
+	ensures output.Success? ==> GetParametersForImportSucceededWith (  input , output.value )
+ method {:extern} GetPublicKey ( input: GetPublicKeyRequest ) returns (output: Result<GetPublicKeyResponse, Error>)
+	ensures GetPublicKeyCalledWith (  input )
+	ensures output.Success? ==> GetPublicKeySucceededWith (  input , output.value )
+ method {:extern} ImportKeyMaterial ( input: ImportKeyMaterialRequest ) returns (output: Result<ImportKeyMaterialResponse, Error>)
+	ensures ImportKeyMaterialCalledWith (  input )
+	ensures output.Success? ==> ImportKeyMaterialSucceededWith (  input , output.value )
+ method {:extern} ListAliases ( input: ListAliasesRequest ) returns (output: Result<ListAliasesResponse, Error>)
+	ensures ListAliasesCalledWith (  input )
+	ensures output.Success? ==> ListAliasesSucceededWith (  input , output.value )
+ method {:extern} ListGrants ( input: ListGrantsRequest ) returns (output: Result<ListGrantsResponse, Error>)
+	ensures ListGrantsCalledWith (  input )
+	ensures output.Success? ==> ListGrantsSucceededWith (  input , output.value )
+ method {:extern} ListKeyPolicies ( input: ListKeyPoliciesRequest ) returns (output: Result<ListKeyPoliciesResponse, Error>)
+	ensures ListKeyPoliciesCalledWith (  input )
+	ensures output.Success? ==> ListKeyPoliciesSucceededWith (  input , output.value )
+ method {:extern} ListResourceTags ( input: ListResourceTagsRequest ) returns (output: Result<ListResourceTagsResponse, Error>)
+	ensures ListResourceTagsCalledWith (  input )
+	ensures output.Success? ==> ListResourceTagsSucceededWith (  input , output.value )
+ method {:extern} PutKeyPolicy ( input: PutKeyPolicyRequest ) returns (output: Result<(), Error>)
+	ensures PutKeyPolicyCalledWith (  input )
+	ensures output.Success? ==> PutKeyPolicySucceededWith (  input )
+ method {:extern} ReEncrypt ( input: ReEncryptRequest ) returns (output: Result<ReEncryptResponse, Error>)
+	ensures ReEncryptCalledWith (  input )
+	ensures output.Success? ==> ReEncryptSucceededWith (  input , output.value )
+ method {:extern} ReplicateKey ( input: ReplicateKeyRequest ) returns (output: Result<ReplicateKeyResponse, Error>)
+	ensures ReplicateKeyCalledWith (  input )
+	ensures output.Success? ==> ReplicateKeySucceededWith (  input , output.value )
+ method {:extern} RetireGrant ( input: RetireGrantRequest ) returns (output: Result<(), Error>)
+	ensures RetireGrantCalledWith (  input )
+	ensures output.Success? ==> RetireGrantSucceededWith (  input )
+ method {:extern} RevokeGrant ( input: RevokeGrantRequest ) returns (output: Result<(), Error>)
+	ensures RevokeGrantCalledWith (  input )
+	ensures output.Success? ==> RevokeGrantSucceededWith (  input )
+ method {:extern} ScheduleKeyDeletion ( input: ScheduleKeyDeletionRequest ) returns (output: Result<ScheduleKeyDeletionResponse, Error>)
+	ensures ScheduleKeyDeletionCalledWith (  input )
+	ensures output.Success? ==> ScheduleKeyDeletionSucceededWith (  input , output.value )
+ method {:extern} Sign ( input: SignRequest ) returns (output: Result<SignResponse, Error>)
+	ensures SignCalledWith (  input )
+	ensures output.Success? ==> SignSucceededWith (  input , output.value )
+ method {:extern} TagResource ( input: TagResourceRequest ) returns (output: Result<(), Error>)
+	ensures TagResourceCalledWith (  input )
+	ensures output.Success? ==> TagResourceSucceededWith (  input )
+ method {:extern} UntagResource ( input: UntagResourceRequest ) returns (output: Result<(), Error>)
+	ensures UntagResourceCalledWith (  input )
+	ensures output.Success? ==> UntagResourceSucceededWith (  input )
+ method {:extern} UpdateAlias ( input: UpdateAliasRequest ) returns (output: Result<(), Error>)
+	ensures UpdateAliasCalledWith (  input )
+	ensures output.Success? ==> UpdateAliasSucceededWith (  input )
+ method {:extern} UpdateCustomKeyStore ( input: UpdateCustomKeyStoreRequest ) returns (output: Result<UpdateCustomKeyStoreResponse, Error>)
+	ensures UpdateCustomKeyStoreCalledWith (  input )
+	ensures output.Success? ==> UpdateCustomKeyStoreSucceededWith (  input , output.value )
+ method {:extern} UpdateKeyDescription ( input: UpdateKeyDescriptionRequest ) returns (output: Result<(), Error>)
+	ensures UpdateKeyDescriptionCalledWith (  input )
+	ensures output.Success? ==> UpdateKeyDescriptionSucceededWith (  input )
+ method {:extern} UpdatePrimaryRegion ( input: UpdatePrimaryRegionRequest ) returns (output: Result<(), Error>)
+	ensures UpdatePrimaryRegionCalledWith (  input )
+	ensures output.Success? ==> UpdatePrimaryRegionSucceededWith (  input )
+ method {:extern} Verify ( input: VerifyRequest ) returns (output: Result<VerifyResponse, Error>)
+	ensures VerifyCalledWith (  input )
+	ensures output.Success? ==> VerifySucceededWith (  input , output.value )
+}
 }
